@prefix ex:    <http://example.com/ns#> .
@prefix rdf:   <http://www.w3.org/1999/02/22-rdf-syntax-ns#> .
@prefix sh:    <http://www.w3.org/ns/shacl#> .
@prefix owl:   <http://www.w3.org/2002/07/owl#> .
@prefix xsd:   <http://www.w3.org/2001/XMLSchema#> .
@prefix rdfs:  <http://www.w3.org/2000/01/rdf-schema#> .

ex:PropertyCommentShape
        rdf:type        sh:NodeShape ;
        rdfs:comment    "Each rdf:Property, owl:DatatypeProperty or owl:ObjectProperty must have at least one rdfs:label" ;
        rdfs:label      "Properties must have a comment" ;
        sh:property     [ sh:datatype  rdf:langString ;
                          sh:minCount  1 ;
                          sh:path      rdfs:comment
                        ] ;
        sh:targetClass  owl:ObjectProperty , owl:DatatypeProperty , rdf:Property .

ex:PropertyNoSuperpropertyShape
        rdf:type        sh:NodeShape ;
        rdfs:comment    "Each rdf:Property, owl:DatatypeProperty or owl:ObjectProperty must have at most one superproperty" ;
        rdfs:label      "Properties must have at most one superproperty" ;
        sh:property     [ sh:maxCount  1 ;
                          sh:path      rdfs:subPropertyOf
                        ] ;
        sh:targetClass  owl:ObjectProperty , owl:DatatypeProperty , rdf:Property .

ex:NamespacePersistentShape
        rdf:type        sh:NodeShape ;
        rdfs:comment    "Namespaces should be called via purl.org or w3id.org" ;
        rdfs:label      "Namespaces should be persistent" ;
        sh:or           ( [ sh:pattern  ".*purl.org.*" ]
                          [ sh:pattern  ".*w3id.org.*" ]
                        ) ;
        sh:targetClass  owl:Ontology .

ex:ClassNoSynonymShape
        rdf:type        sh:NodeShape ;
        rdfs:comment    "No owl:equivalentClass relationship is allowed between two owl:Class within the same namespace" ;
        rdfs:label      "Detect synonyms created as classes" ;
        sh:sparql       [ sh:select  "\n    SELECT $this\n    WHERE {\n    $this a owl:Class .\n    $this owl:equivalentClass ?other\n    BIND(REPLACE(STR($this), '(#|/)[^#/]*$', '$1' ) as ?ns1) .\n    BIND(REPLACE(STR(?other), '(#|/)[^#/]*$', '$1' ) as ?ns2) .\n    FILTER(?ns1 = ?ns2) .\n    }\n    " ] ;
        sh:targetClass  owl:Class .

ex:ClassLabelShape  rdf:type  sh:NodeShape ;
        rdfs:comment    "A class must at least have one label" ;
        rdfs:label      "Label shape" ;
        sh:property     [ sh:datatype  rdf:langString ;
                          sh:minCount  1 ;
                          sh:path      rdfs:label
                        ] ;
        sh:targetClass  owl:Class .

ex:ClassNoLowercaseShape
        rdf:type        sh:NodeShape ;
        rdfs:comment    "For naming conventions, each owl:Class name must not start with a lowercase letter" ;
        rdfs:label      "Classes names must not start with a lowercase letter" ;
        sh:sparql       [ sh:select  "\n    SELECT $this\n    WHERE {\n    $this a owl:Class .\n    BIND(REPLACE(STR($this), '/([a-z][1]?[A-z0-9]*)$', '' ) as ?str1) .\n    FILTER(STR($this) != STR(?str1)) .\n    }\n    " ] ;
        sh:targetClass  owl:Class .

ex:PropertyNoInverseShape
        rdf:type        sh:NodeShape ;
        rdfs:comment    "Check if any rdf:Property, owl:DatatypeProperty or owl:ObjectProperty is owl:inverseOf of itself." ;
        rdfs:label      "Detect relationships inverse to themselves" ;
        sh:sparql       [ sh:select  "\n    SELECT $this\n    WHERE {\n    $this a ?property .\n    $this owl:inverseOf $this .\n    FILTER(?property IN (rdf:Property, owl:DatatypeProperty, owl:ObjectProperty)) .\n    }\n    " ] ;
        sh:targetClass  owl:ObjectProperty , owl:DatatypeProperty , rdf:Property .

ex:PropertyNoCapitaLetterShape
        rdf:type        sh:NodeShape ;
        rdfs:comment    "For naming conventions, each rdf:Property, owl:DatatypeProperty or owl:ObjectProperty name must not start with a capital letter" ;
        rdfs:label      "Properties names must not start with a capital letter" ;
        sh:sparql       [ sh:select  "\n    SELECT $this\n    WHERE {\n    $this a ?property .\n    FILTER(?property IN (rdf:Property, owl:DatatypeProperty, owl:ObjectProperty)) .\n    BIND(REPLACE(STR($this), '/[A-Z][A-z0-9]*$', '' ) as ?str1) .\n    FILTER(STR($this) != STR(?str1)) .\n    }\n    " ] ;
        sh:targetClass  owl:ObjectProperty , owl:DatatypeProperty , rdf:Property .

ex:SuperclassShape  rdf:type  sh:NodeShape ;
        rdfs:comment    "Each class must have at most one superclass." ;
        rdfs:label      "Superclass shape" ;
        sh:sparql       [ rdf:type     sh:SPARQLConstraint ;
                          sh:prefixes  [ sh:declare  [ sh:namespace  "http://www.w3.org/2000/01/rdf-schema##" ;
                                                       sh:prefix     "rdfs"
                                                     ] ;
                                         sh:declare  [ sh:namespace  "http://www.w3.org/1999/02/22-rdf-syntax-ns#" ;
                                                       sh:prefix     "rdf"
                                                     ]
                                       ] ;
                          sh:select    "\n    SELECT DISTINCT $this\n    WHERE {\n    $this rdf:type owl:Class .\n    $this rdfs:subClassOf ?v1 .\n    $this rdfs:subClassOf ?v2 .\n    FILTER NOT EXISTS {?v1 rdfs:subClassOf ?v2 }.\n    FILTER NOT EXISTS {?v2 rdfs:subClassOf ?v1 }.\n    FILTER(?v1 != ?v2) .\n    FILTER(?v1 != owl:Thing) .\n    FILTER(?v2 != owl:Thing) .\n    FILTER($this != ?v1) .\n    FILTER($this != ?v2) .\n    }\n    "
                        ] ;
        sh:targetClass  owl:Class .

ex:ClassCommentShape  rdf:type  sh:NodeShape ;
        rdfs:comment    "Each owl:Class must have at least one rdfs:comment, which must be unique for each language." ;
        rdfs:label      "Classes must have a comment" ;
        sh:property     [ sh:datatype  rdf:langString ;
                          sh:minCount  1 ;
                          sh:path      rdfs:comment
                        ] ;
        sh:targetClass  owl:Class .

ex:ClassConnectedShape
        rdf:type        sh:NodeShape ;
        rdfs:comment    "Check whether a owl:Class (a) is not part of any hierarchy (using rdfs:subClassOf) (b) does not have any definition axiom (using rdfs:subClassOf or owl:equivalentClass and a class restriction expression) (c) does not appear in any other class definition axiom (using rdfs:subClassOf or owl:equivalentClass and a class restriction expression) (d) does not appear in any rdfs:domain or rdfs:range." ;
        rdfs:label      "Detect unconnected classes" ;
        sh:sparql       [ sh:select  "\n    SELECT $this WHERE\n    {\n    $this a owl:Class .\n    FILTER NOT EXISTS {$this rdfs:subClassOf ?any1} .\n    FILTER NOT EXISTS {?any2 owl:equivalentClass $this} .\n    FILTER NOT EXISTS {$this owl:equivalentClass ?any3} .\n    FILTER NOT EXISTS {?any4 rdfs:subClassOf $this} .\n    FILTER NOT EXISTS {?any5 rdfs:range $this} .\n    FILTER NOT EXISTS {?any6 rdfs:domain $this} .\n    }\n    " ] ;
        sh:targetClass  owl:Class .

ex:ClassCyclesShape  rdf:type  sh:NodeShape ;
        rdfs:comment    "No owl:Class can be rdfs:subClassOf itself in any level" ;
        rdfs:label      "Detect cycles in the class hierarchy" ;
        sh:sparql       [ sh:select  "\n    SELECT $this WHERE\n    {\n    $this a owl:Class .\n    $this rdfs:subClassOf+ $this .\n    }\n    " ] ;
        sh:targetClass  owl:Class .

ex:PropertyLabelShape
        rdf:type        sh:NodeShape ;
        rdfs:comment    "Each rdf:Property, owl:DatatypeProperty or owl:ObjectProperty must have at least one rdfs:label" ;
        rdfs:label      "Properties must have a label" ;
        sh:property     [ sh:datatype  rdf:langString ;
                          sh:minCount  1 ;
                          sh:path      rdfs:label
                        ] ;
        sh:targetClass  owl:ObjectProperty , owl:DatatypeProperty , rdf:Property .
