@prefix :      <https://w3id.org/steel/ProcessOntology/> .
@prefix rr:    <http://www.w3.org/ns/r2rml#> .
@prefix grel:  <http://users.ugent.be/~bjdmeest/function/grel.ttl#> .
@prefix d2rq:  <http://www.wiwiss.fu-berlin.de/suhl/bizer/D2RQ/0.1#> .
@prefix void:  <http://rdfs.org/ns/void#> .
@prefix owl:   <http://www.w3.org/2002/07/owl#> .
@prefix emmo:  <http://emmo.info/emmo#> .
@prefix fno:   <https://w3id.org/function/ontology#> .
@prefix xsd:   <http://www.w3.org/2001/XMLSchema#> .
@prefix skos:  <http://www.w3.org/2004/02/skos/core#> .
@prefix rdfs:  <http://www.w3.org/2000/01/rdf-schema#> .
@prefix pmdco: <https://material-digital.de/pmdco/> .
@prefix rml:   <http://semweb.mmlab.be/ns/rml#> .
@prefix sfunc: <http://w3id.org/steel/xlsx2owl-utils/functions.ttl#> .
@prefix rdf:   <http://www.w3.org/1999/02/22-rdf-syntax-ns#> .
@prefix fnml:  <http://semweb.mmlab.be/ns/fnml#> .
@prefix ql:    <http://semweb.mmlab.be/ns/ql#> .
@prefix foaf:  <http://xmlns.com/foaf/0.1/> .
@prefix dc:    <http://purl.org/dc/elements/1.1/> .

:output  rdf:type       owl:DatatypeProperty ;
        rdfs:domain     :Workflow ;
        rdfs:label      "output"@en ;
        skos:preflabel  "output"@en .

:MaterialIdentifier  rdf:type  skos:Concept , owl:Class ;
        rdfs:comment       "Material identification for which this erosion definition applies.A unique number or label must be specified"@en , "A unique number or label to address the defined material"@en ;
        rdfs:label         "MaterialIdentifier"@en ;
        rdfs:subClassOf    "https://material-digital.de/pmdco/ValueObject" ;
        skos:altlabel      "MID"@en ;
        skos:preflabel     "MaterialIdentifier"@en ;
        :UnitLabel         "-" ;
        :hasLabelSourceEn  "LS-DYNA_Manual_Volume_2" .

:hasFailureStrainIdentifier4StrainRate
        rdf:type        owl:ObjectProperty ;
        rdfs:label      "hasFailureStrainIdentifier4StrainRate"@en ;
        rdfs:range      "https://w3id.org/steel/ProcessOntology/FailureStrainIdentifier4StrainRate" ;
        skos:preflabel  "hasFailureStrainIdentifier4StrainRate"@en .

:ProjectNumber  rdf:type  skos:Concept , owl:Class ;
        rdfs:comment    "Project identification number."@en ;
        rdfs:label      "ProjectNumber"@en ;
        skos:altlabel   "Projektnummer"@de , "Project number"@en ;
        skos:preflabel  "ProjectNumber"@en .

:ExtensometerGaugeLength
        rdf:type        skos:Concept , owl:Class ;
        rdfs:comment    "The intial gauge length Le used for measurement of extension by means of an extensometer"@en , "The intial gauge length used for measurement of extension by means of an extensometer"@en ;
        rdfs:label      "ExtensometerGaugeLength"@en ;
        skos:altlabel   "extensometer gauge length"@en , "Extensometer gauge length "@en , "Messlänge L0"@de , "Messlänge Lo"@de ;
        skos:preflabel  "ExtensometerGaugeLength"@en .

:FinalGaugeLengthAfterFracture
        rdf:type        skos:Concept , owl:Class ;
        rdfs:comment    "Länge zwischen den Marken zur Kennzeichnung der Messlänge (3.1) auf der Probe, die nach dem Bruch bei Raumtemperatur gemessen wird, nachdem die beiden Probenbruchstücke sorgfältig so zusammengefügt wurden, dass ihre Achsen in einer Geraden liegen"@de ;
        rdfs:label      "FinalGaugeLengthAfterFracture"@en ;
        skos:altlabel   "final gauge length after fracture"@en ;
        skos:preflabel  "FinalGaugeLengthAfterFracture"@en .

:Texture  rdf:type      owl:Class ;
        rdfs:label      "Texture"@en , "Textur"@de ;
        skos:altlabel   "Oberflächenbeschaffenheit"@de ;
        skos:preflabel  "Texture"@en , "Textur"@de .

:related  rdf:type      owl:ObjectProperty ;
        rdfs:label      "is related to"@en ;
        dc:description  "some things are related"@en ;
        skos:preflabel  "is related to"@en .

:hasFailureCriteriaTypeAdd4StrainAverage
        rdf:type        owl:ObjectProperty ;
        rdfs:label      "hasFailureCriteriaTypeAdd4StrainAverage"@en ;
        rdfs:range      "https://w3id.org/steel/ProcessOntology/FailureCriteriaTypeAdd4StrainAverage" ;
        skos:preflabel  "hasFailureCriteriaTypeAdd4StrainAverage"@en .

:ressourceUri  rdf:type  owl:DatatypeProperty ;
        rdfs:domain     :CodeFileRessource ;
        rdfs:label      "uri"@en ;
        rdfs:range      xsd:string ;
        skos:preflabel  "uri"@en .

:TimeStamp  rdf:type    skos:Concept , owl:Class ;
        rdfs:comment    "Date and time when the experiment was conducted."@en , "Date when the experiment was conducted."@en ;
        rdfs:label      "TimeStamp"@en ;
        skos:altlabel   "Date"@en , "Date/Time"@en , "Datum/Uhrzeit"@de , "Datum"@de ;
        skos:preflabel  "TimeStamp"@en .

:ForceTransducer  rdf:type  skos:Concept , owl:Class ;
        rdfs:comment    "Die Kraftmesseinrichtung der Zugprüfmaschine muss im relevanten Bereich mindestens der Klasse 1 nach ISO 7500-1 entsprechen."@de ;
        rdfs:label      "ForceTransducer"@en ;
        skos:preflabel  "ForceTransducer"@en .

<https://w3id.org/steel/ProcessOntology>
        rdf:type         owl:Ontology ;
        rdfs:label       "StahlDigital Vocabulary"@en ;
        dc:description   "Vocabulary of project StahlDigital"@en ;
        owl:versionInfo  "0.1 (preliminary)"@en ;
        skos:prefLabel   "StahlDigital Vocabulary"@en ;
        foaf:depiction   :graph.png .

:GrainOrientation  rdf:type  owl:Class ;
        rdfs:label      "grain orientation"@en , "Kornausrichtung"@de ;
        skos:preflabel  "grain orientation"@en , "Kornausrichtung"@de .

:TimeSeriesSimulation
        rdf:type        owl:Class ;
        rdfs:comment    "A Simulation that return a time Series"@en ;
        rdfs:label      "Zeitreihensimulation"@de , "Time series simulation"@en ;
        skos:preflabel  "Zeitreihensimulation"@de , "Time series simulation"@en .

:Tester  rdf:type       skos:Concept , owl:Class ;
        rdfs:comment    "The name or ID of the person who conducted the experiment."@en ;
        rdfs:label      "Tester"@en ;
        skos:altlabel   "Tester"@en , "Prüfer"@de ;
        skos:preflabel  "Tester"@en .

:ProofStrength_0.2Percentage
        rdf:type        skos:Concept , owl:Class ;
        rdfs:comment    "yield strength, 0.2 %"@en ;
        rdfs:label      "ProofStrength_0.2Percentage"@en ;
        skos:altlabel   "proof strength, 0.2 %"@en , "Rp0.2"@de ;
        skos:preflabel  "ProofStrength_0.2Percentage"@en .

:FrameOfReference  rdf:type  owl:Class ;
        rdfs:label      "Referenzrahmen"@de , "Frame of reference"@en ;
        skos:preflabel  "Referenzrahmen"@de , "Frame of reference"@en .

:TestPieceGeometry  rdf:type  skos:Concept , owl:Class ;
        rdfs:comment    "The type of the specimen."@en ;
        rdfs:label      "TestPieceGeometry"@en ;
        skos:altlabel   "Test piece geometry"@en , "Specimen type"@en , "Probentyp"@de , "Probenform"@de ;
        skos:preflabel  "TestPieceGeometry"@en .

:TrueStrain  rdf:type   owl:Class , skos:Concept ;
        rdfs:comment    "true strain"@en ;
        rdfs:label      "True Strain"@en , "TrueStrain"@en , "wahre Dehnung"@de ;
        skos:altlabel   "epsw(dL)"@de , "true strain"@en ;
        skos:preflabel  "True Strain"@en , "wahre Dehnung"@de , "TrueStrain"@en .

:Composition  rdf:type  owl:Class ;
        rdfs:comment    "Combination of Elements in a Phase or a whole Sample. Related to Alloys"@en ;
        rdfs:label      "Zusammensetzung"@de , "Composition"@en ;
        skos:altlabel   "alloy"@en , "Legierung"@de ;
        skos:preflabel  "Zusammensetzung"@de , "Composition"@en .

:hasStrainRateScaleParameterC
        rdf:type        owl:ObjectProperty ;
        rdfs:label      "hasStrainRateScaleParameterC"@en ;
        rdfs:range      "https://w3id.org/steel/ProcessOntology/StrainRateScaleParameterC" ;
        skos:preflabel  "hasStrainRateScaleParameterC"@en .

:StrainRateScaleParameterP
        rdf:type           skos:Concept , owl:Class ;
        rdfs:comment       "Parameter P for strain rate approach for using the Cowper and Symonds model which scales the yield stress with the factor: 1+(epsDot/C)^(1/P)"@en ;
        rdfs:label         "StrainRateScaleParameterP"@en ;
        rdfs:subClassOf    "https://material-digital.de/pmdco/ValueObject" ;
        skos:altlabel      "P"@en ;
        skos:preflabel     "StrainRateScaleParameterP"@en ;
        :UnitLabel         "1" ;
        :hasLabelSourceEn  "LS-DYNA_Manual_Volume_2" .

:NakajimaTest  rdf:type  owl:Class ;
        rdfs:label       "Nakajima Test"@en , "Nakajima Test"@de ;
        rdfs:subClassOf  :ExperimentalTest ;
        skos:preflabel   "Nakajima Test"@en , "Nakajima Test"@de .

:workflowSteps  rdf:type  owl:DatatypeProperty ;
        rdfs:domain     :Workflow ;
        rdfs:label      "steps"@en ;
        dc:description  "operations on data, can be other workflows, has pervious and following step"@en ;
        skos:preflabel  "steps"@en .

:Component  rdf:type    owl:Class ;
        rdfs:label      "Komponente"@de , "Component"@en ;
        skos:preflabel  "Komponente"@de , "Component"@en .

:CrossheadDisplacement
        rdf:type        skos:Concept , owl:Class ;
        rdfs:comment    "Displacement of the actuator"@en ;
        rdfs:label      "CrossheadDisplacement"@en ;
        skos:altlabel   "Maschine"@de , "Crosshead displacement"@en ;
        skos:preflabel  "CrossheadDisplacement"@en .

:MAT_ADD_DAMAGE_GISSMO
        rdf:type           skos:Concept , owl:Class ;
        rdfs:label         "MAT_ADD_DAMAGE_GISSMO"@en ;
        rdfs:subClassOf    "https://material-digital.de/pmdco/ValueObject" ;
        skos:preflabel     "MAT_ADD_DAMAGE_GISSMO"@en ;
        :hasLabelSourceEn  "LS-DYNA_Manual_Volume_2" .

:Microstructure  rdf:type  owl:Class ;
        rdfs:label      "Microstructure"@en , "Gefüge"@de ;
        skos:preflabel  "Microstructure"@en , "Gefüge"@de .

:Elongation  rdf:type   skos:Concept , owl:Class ;
        rdfs:comment    "Zunahme der Anfangsmesslänge (3.1.1) zu einem beliebigen Zeitpunkt während des Versuchs"@de , "Verlängerung (3.3), angegeben in Prozent, bezogen auf die Anfangsmesslänge (3.1.1)"@de ;
        rdfs:label      "Elongation"@en , "Dehnung"@de ;
        skos:altlabel   "elongation"@en ;
        skos:preflabel  "Elongation"@en , "Dehnung"@de .

:hasFailureTreatment  rdf:type  owl:ObjectProperty ;
        rdfs:label      "hasFailureTreatment"@en ;
        rdfs:range      "https://w3id.org/steel/ProcessOntology/FailureTreatment" ;
        skos:preflabel  "hasFailureTreatment"@en .

:Phase  rdf:type        owl:Class ;
        rdfs:comment    "Region of space (a thermodynamic system), throughout which all physical properties of a material are essentially uniform (Wikipedia)"@en ;
        rdfs:label      "Phase"@en , "Phase"@de ;
        skos:preflabel  "Phase"@en , "Phase"@de .

:CrossheadSeparationRate
        rdf:type        skos:Concept , owl:Class ;
        rdfs:comment    "The displacement of the crosshead per time"@en , "The speed of the experiment."@en ;
        rdfs:label      "CrossheadSeparationRate"@en ;
        skos:altlabel   "Test speed"@en , "Prüfgeschwindigkeit"@de , "crosshead separation rate"@en , "Crosshead separation rate vc"@en ;
        skos:preflabel  "CrossheadSeparationRate"@en .

:TrueStressAtFracture
        rdf:type        skos:Concept , owl:Class ;
        rdfs:comment    "true stress at fracture"@en ;
        rdfs:label      "TrueStressAtFracture"@en ;
        skos:altlabel   "wahre Bruchspannung"@de , "True stress at fracture"@en ;
        skos:preflabel  "TrueStressAtFracture"@en .

:hasReferenceTemperature
        rdf:type        owl:ObjectProperty ;
        rdfs:label      "hasReferenceTemperature"@en ;
        rdfs:range      "https://w3id.org/steel/ProcessOntology/ReferenceTemperature" ;
        skos:preflabel  "hasReferenceTemperature"@en .

:TimeIncrementStep  rdf:type  owl:Class ;
        rdfs:label      "time increment step"@en ;
        skos:preflabel  "time increment step"@en .

:input  rdf:type        owl:DatatypeProperty ;
        rdfs:domain     :Workflow ;
        rdfs:label      "input"@en ;
        skos:preflabel  "input"@en .

:FailureTreatment  rdf:type  skos:Concept , owl:Class ;
        rdfs:comment       "Descibes the treatment of failure:\n<0…User defined failure subroutine, matusr_24 in dyn21.F\n=0…no failure is taken into account\n>0…constant failure strain"@en ;
        rdfs:label         "FailureTreatment"@en ;
        rdfs:subClassOf    "https://material-digital.de/pmdco/ValueObject" ;
        skos:altlabel      "FAIL"@en ;
        skos:preflabel     "FailureTreatment"@en ;
        :UnitLabel         "1" ;
        :hasLabelSourceEn  "LS-DYNA_Manual_Volume_2" .

:ProofStrength_1Percentage
        rdf:type        skos:Concept , owl:Class ;
        rdfs:comment    "yield strength, 1 %"@en ;
        rdfs:label      "ProofStrength_1Percentage"@en ;
        skos:altlabel   "proof strength, 1 %"@en , "Rp1"@de ;
        skos:preflabel  "ProofStrength_1Percentage"@en .

:norm   rdf:type        owl:DatatypeProperty ;
        rdfs:label      "norm"@en ;
        dc:description  "The norm according to which the experiment was conducted."@en ;
        skos:preflabel  "norm"@en .

:PercentagePermanentExtension
        rdf:type        skos:Concept , owl:Class ;
        rdfs:comment    "plastic engineering strain"@en ;
        rdfs:label      "PercentagePermanentExtension"@en ;
        skos:altlabel   "percentage permanent extension "@en , "percentage permanent extension"@en , "eps-plast"@de , "e-plast"@de ;
        skos:preflabel  "PercentagePermanentExtension"@en .

:Time   rdf:type        skos:Concept , owl:Class ;
        rdfs:comment    "Authors"@de , "The time when the data point is recorded in relation to the start. "@en , "0.694"@en ;
        rdfs:label      "Time"@en ;
        skos:altlabel   "Zeit"@de , "Time"@en , "Test time"@en , "Prüfzeit"@de ;
        skos:preflabel  "Time"@en .

:hasPoissonRatio  rdf:type  owl:ObjectProperty ;
        rdfs:label      "hasPoissonRatio"@en ;
        rdfs:range      "https://w3id.org/steel/ProcessOntology/PoissonRatio" ;
        skos:preflabel  "hasPoissonRatio"@en .

:Material  rdf:type     skos:Concept , owl:Class ;
        rdfs:comment    "The material used in the experiment."@en ;
        rdfs:label      "Material"@en ;
        skos:altlabel   "material"@en , "Werkstoff"@de , "Material"@en ;
        skos:preflabel  "Material"@en .

:HDF5   rdf:type        owl:Class ;
        rdfs:label      "HDF5 File Format"@en , "HDF5 Dateiformat"@de ;
        skos:preflabel  "HDF5 File Format"@en , "HDF5 Dateiformat"@de .

<https://w3id.org/steel/ProcessOntology/ProofStrength%2CTotalExtension>
        rdf:type        skos:Concept , owl:Class ;
        rdfs:label      "ProofStrength,TotalExtension"@en ;
        skos:altlabel   "proof strength, total extension"@en ;
        skos:preflabel  "ProofStrength,TotalExtension"@en .

:hasTangentYieldModulus
        rdf:type        owl:ObjectProperty ;
        rdfs:label      "hasTangentYieldModulus"@en ;
        rdfs:range      "https://w3id.org/steel/ProcessOntology/TangentYieldModulus" ;
        skos:preflabel  "hasTangentYieldModulus"@en .

:NumberFailedIntegrationPoints
        rdf:type           skos:Concept , owl:Class ;
        rdfs:comment       "Number or percentage of failed integration points prior to element deletion.\nGT.0.0: Number of integration points which must fail before element is deleted.\nLT.0.0: Applies only to shells. |NUMFIP| is the percentage of layers which must fail before an element is deleted. For shell formulations with 4 integration points per layer, the layer is considered failed if any of the integration points in the layer fails."@en ;
        rdfs:label         "NumberFailedIntegrationPoints"@en ;
        rdfs:subClassOf    "https://material-digital.de/pmdco/ValueObject" ;
        skos:altlabel      "NUMFIP"@en ;
        skos:preflabel     "NumberFailedIntegrationPoints"@en ;
        :UnitLabel         "1" ;
        :hasLabelSourceEn  "LS-DYNA_Manual_Volume_2" .

:FailureCriteriaTypeAdd
        rdf:type           skos:Concept , owl:Class ;
        rdfs:comment       "Flag for additional failure criterion F2:\n=0.0: off (default)\n=1.0: on; An additional, load-path independent, failure criterion can be invoked, where the current state of plastic strain is used"@en ;
        rdfs:label         "FailureCriteriaTypeAdd"@en ;
        rdfs:subClassOf    "https://material-digital.de/pmdco/ValueObject" ;
        skos:altlabel      "FAILOPT"@en ;
        skos:preflabel     "FailureCriteriaTypeAdd"@en ;
        :UnitLabel         "-" ;
        :hasLabelSourceEn  "LS-DYNA_Manual_Volume_2" .

:hasYoungsModulus  rdf:type  owl:ObjectProperty ;
        rdfs:label      "hasYoungsModulus"@en ;
        rdfs:range      "https://w3id.org/steel/ProcessOntology/YoungsModulus" ;
        skos:preflabel  "hasYoungsModulus"@en .

:TestStandard  rdf:type  skos:Concept , owl:Class ;
        rdfs:comment    "The norm according to which the experiment was conducted."@en ;
        rdfs:label      "TestStandard"@en ;
        skos:altlabel   "Test standard"@en , "Prüfnorm"@de ;
        skos:preflabel  "TestStandard"@en .

:ComponentTest  rdf:type  owl:Class ;
        rdfs:label      "Komponententest"@de , "Component test"@en ;
        skos:preflabel  "Komponententest"@de , "Component test"@en .

:FailureStrainIdentifier4MeshDependency
        rdf:type           skos:Concept , owl:Class ;
        rdfs:comment       "The load curve ID defines plastic failure strain as a function of element size. The table ID defines for each triaxiality a load curve ID giving the plastic failure strain versus element size for that triaxiality. If a three dimensional table ID is referred, plastic failure strain can be a function of Lode parameter (TABLE_\n3D), triaxiality (TABLE), and element size (CURVE)"@en ;
        rdfs:label         "FailureStrainIdentifier4MeshDependency"@en ;
        rdfs:subClassOf    "https://material-digital.de/pmdco/ValueObject" ;
        skos:altlabel      "LCI"@en ;
        skos:preflabel     "FailureStrainIdentifier4MeshDependency"@en ;
        :UnitLabel         "-" ;
        :hasLabelSourceEn  "LS-DYNA_Manual_Volume_2" .

:Force  rdf:type        owl:Class , skos:Concept ;
        rdfs:comment    "The force measured by the load cell"@en , "The force that is measured using the Force-measuring device."@en , "The force measured with the force measuring system"@en ;
        rdfs:label      "Force"@en , "Kraft"@de ;
        skos:altlabel   "Standardkraft"@de , "F"@de , "Standard force"@en , "Force"@en , "Force-measuring device"@en ;
        skos:preflabel  "Force"@en , "Kraft"@de .

:RollingDirection  rdf:type  skos:Concept , owl:Class ;
        rdfs:label      "RollingDirection"@en ;
        skos:altlabel   "Walzrichtung"@de ;
        skos:preflabel  "RollingDirection"@en .

:Software  rdf:type     owl:Class ;
        rdfs:label      "software"@en , "Software"@de ;
        skos:altlabel   "Programm"@de ;
        skos:preflabel  "software"@en , "Software"@de .

:PropertyOfStructuralRelevance
        rdf:type        owl:Class ;
        rdfs:comment    "Properties that contribute towards the structural integrity of a component. Example Thickness, negative example Paint/ Color of Paint"@en ;
        rdfs:label      "Strukturrelevante Eigenschaft"@de , "Property of structural relevance"@en ;
        skos:preflabel  "Strukturrelevante Eigenschaft"@de , "Property of structural relevance"@en .

:EngineeringStress  rdf:type  skos:Concept , owl:Class ;
        rdfs:label      "EngineeringStress"@en ;
        skos:altlabel   "engineering stress"@en , "Sigma-technisch"@de ;
        skos:preflabel  "EngineeringStress"@en .

:TestSpeed  rdf:type    skos:Concept , owl:Class ;
        rdfs:comment    "während des Versuchs verwendete Geschwindigkeit(en)"@de ;
        rdfs:label      "TestSpeed"@en ;
        skos:preflabel  "TestSpeed"@en .

:PercentageReductionOfArea
        rdf:type        skos:Concept , owl:Class ;
        rdfs:comment    "maximum change in cross-sectional area which has occured during the test expressed as a percentage of the original cross-sectional area"@en ;
        rdfs:label      "PercentageReductionOfArea"@en ;
        skos:altlabel   "percentage reduction of area"@en , "Z"@de , "Brucheinschnürung Z"@de ;
        skos:preflabel  "PercentageReductionOfArea"@en .

:TimeSeries  rdf:type   owl:Class ;
        rdfs:label      "Zeitreihe"@de , "Time series"@en ;
        skos:preflabel  "Zeitreihe"@de , "Time series"@en .

:FrameRate  rdf:type    skos:Concept , owl:Class ;
        rdfs:comment    "sampling rate of the strain measuring system (e.g. high speed video recording)"@en ;
        rdfs:label      "FrameRate"@en ;
        skos:altlabel   "Frame rate"@en , "Abtastrate"@de ;
        skos:preflabel  "FrameRate"@en .

:Job    rdf:type        owl:Class ;
        rdfs:label      "Job"@en , "Job"@de ;
        skos:altlabel   "Execution Job"@en ;
        skos:preflabel  "Job"@en , "Job"@de .

:TotalElongation  rdf:type  owl:Class ;
        rdfs:label      "Total Elongation"@en , "Bruchdehnung"@de ;
        skos:preflabel  "Total Elongation"@en , "Bruchdehnung"@de .

:DefaultValue  rdf:type  skos:Concept , owl:Class ;
        rdfs:label      "DefaultValue"@en ;
        skos:altlabel   "default value"@en ;
        skos:preflabel  "DefaultValue"@en .

:Fracture  rdf:type     skos:Concept , owl:Class ;
        rdfs:label      "Fracture"@en ;
        skos:altlabel   "fracture"@en ;
        skos:preflabel  "Fracture"@en .

:CharacteristicEngineeringStrainRate
        rdf:type        skos:Concept , owl:Class ;
        rdfs:comment    "Mean value of the time-dependent engineering strain rate in the range between start of yield or 1% strain and strain at maximum force"@en ;
        rdfs:label      "CharacteristicEngineeringStrainRate"@en ;
        skos:altlabel   "plastische"@de , "Characteristic engineering strain rate"@en ;
        skos:preflabel  "CharacteristicEngineeringStrainRate"@en .

:hasDamageTreatment  rdf:type  owl:ObjectProperty ;
        rdfs:label      "hasDamageTreatment"@en ;
        rdfs:range      "https://w3id.org/steel/ProcessOntology/DamageTreatment" ;
        skos:preflabel  "hasDamageTreatment"@en .

:ReferenceJob  rdf:type  owl:Class ;
        rdfs:comment     "a Pyiron job for ..."@en ;
        rdfs:label       "Reference Job"@en ;
        rdfs:subClassOf  :PyironJob ;
        skos:preflabel   "Reference Job"@en .

:TestPieceLength  rdf:type  skos:Concept , owl:Class ;
        rdfs:label      "TestPieceLength"@en ;
        skos:altlabel   "Test piece length"@en , "Probengesamtlänge Lt"@de ;
        skos:preflabel  "TestPieceLength"@en .

:MechanicalCard  rdf:type  owl:Class ;
        skos:altlabel  "MaterialKarte"@de , "MaterialCard"@en .

:ChemicalComposition  rdf:type  owl:Class ;
        rdfs:label      "Chemische Zusammensetzung"@de , "Chemical Composition"@en ;
        skos:preflabel  "Chemische Zusammensetzung"@de , "Chemical Composition"@en .

:Remark  rdf:type       skos:Concept , owl:Class ;
        rdfs:comment    "A specific comment about the experiment."@en ;
        rdfs:label      "Remark"@en ;
        skos:altlabel   "Remark"@en , "Bemerkungen"@de , "Bemerkung"@de ;
        skos:preflabel  "Remark"@en .

:ConstitutiveModel  rdf:type  owl:Class .

:ModulusOfElasticity  rdf:type  skos:Concept , owl:Class ;
        rdfs:label      "ModulusOfElasticity"@en ;
        skos:altlabel   "modulus of elasticity"@en , "Elastizitätsmodul"@de , "EModul"@de , "E-Modul"@de ;
        skos:preflabel  "ModulusOfElasticity"@en .

:Model  rdf:type        owl:Class ;
        rdfs:label      "Modell"@de , "Model"@en ;
        skos:preflabel  "Modell"@de , "Model"@en .

:UnusualCrashTest  rdf:type  owl:Class ;
        rdfs:comment    "Crashtestresults that differ from simulations"@en ;
        rdfs:label      "Unusual crash test"@en , "Ungewöhnlicher Crashtest"@de ;
        skos:preflabel  "Unusual crash test"@en , "Ungewöhnlicher Crashtest"@de .

:OriginalCrosssection
        rdf:type        skos:Concept , owl:Class ;
        rdfs:comment    "original crosssection area of the parallel length"@en , "Crosssection of the sample."@en , "original cross-sectional area of the parallel length"@en ;
        rdfs:label      "OriginalCrosssection"@en ;
        skos:altlabel   "Original cross section"@en , "Anfangsquerschnitt So"@de , "Querschnitt"@de , "Crosssection"@en , "original cross-sectional area of the parallel length"@en , "So"@de , "Anfangsquerschnitt S0"@de ;
        skos:preflabel  "OriginalCrosssection"@en .

:FractureStress  rdf:type  owl:Class ;
        rdfs:label      "Fracture Stress"@en , "Bruchspannung"@de ;
        skos:preflabel  "Fracture Stress"@en , "Bruchspannung"@de .

:PercentageTotalExtensionAtFracture
        rdf:type        skos:Concept , owl:Class ;
        rdfs:label      "PercentageTotalExtensionAtFracture"@en ;
        skos:altlabel   "percentage total extension at fracture"@en ;
        skos:preflabel  "PercentageTotalExtensionAtFracture"@en .

:hasJob  rdf:type       owl:ObjectProperty ;
        rdfs:domain     :PyironProject ;
        rdfs:label      "has job"@en ;
        rdfs:range      :PyironJob ;
        dc:description  "The relation between pyiron project and jobs"@en ;
        skos:preflabel  "has job"@en .

:ProjectName  rdf:type  skos:Concept , owl:Class ;
        rdfs:comment    "Name of the Project."@en , "Instabilität"@en ;
        rdfs:label      "ProjectName"@en ;
        skos:altlabel   "Projektname"@de , "Project name"@en , "Projekt"@de , "Project"@en ;
        skos:preflabel  "ProjectName"@en .

:hasReferenceElementSize
        rdf:type        owl:ObjectProperty ;
        rdfs:label      "hasReferenceElementSize"@en ;
        rdfs:range      "https://w3id.org/steel/ProcessOntology/ReferenceElementSize" ;
        skos:preflabel  "hasReferenceElementSize"@en .

:Validation  rdf:type   owl:Class ;
        rdfs:label      "Validierung"@de , "Validation"@en ;
        skos:altlabel   "Nachweis"@de , " Gültigkeitserklärung"@de ;
        skos:preflabel  "Validierung"@de , "Validation"@en .

:ScriptJob  rdf:type     owl:Class ;
        rdfs:comment     "a Pyiron job for executing a script like e.g. JupyterNotebook"@en ;
        rdfs:label       "Script Job"@en ;
        rdfs:subClassOf  :PyironJob ;
        skos:preflabel   "Script Job"@en .

:hasMatPiecewiseLinearPlasticity
        rdf:type        owl:ObjectProperty ;
        rdfs:label      "hasMatPiecewiseLinearPlasticity"@en ;
        rdfs:range      "https://w3id.org/steel/ProcessOntology/MatPiecewiseLinearPlasticity" ;
        skos:preflabel  "hasMatPiecewiseLinearPlasticity"@en .

:SpecificHeatCapacity
        rdf:type           skos:Concept , owl:Class ;
        rdfs:comment       "Specific heat capacity"@en ;
        rdfs:label         "SpecificHeatCapacity"@en ;
        rdfs:subClassOf    "https://material-digital.de/pmdco/ValueObject" ;
        skos:altlabel      "CP"@en ;
        skos:preflabel     "SpecificHeatCapacity"@en ;
        :UnitLabel         "J/(g*K)" ;
        :hasLabelSourceEn  "LS-DYNA_Manual_Volume_2" .

:Element  rdf:type      owl:Class ;
        rdfs:comment    "Chemical Elements"@en ;
        rdfs:label      "Element"@en , "Element"@de ;
        skos:altlabel   "chemical elements"@en ;
        skos:preflabel  "Element"@en , "Element"@de .

:Computer-controlledTensileTestingMachine
        rdf:type        skos:Concept , owl:Class ;
        rdfs:label      "Computer-controlledTensileTestingMachine"@en ;
        skos:altlabel   "computer-controlled tensile testing machine"@en ;
        skos:preflabel  "Computer-controlledTensileTestingMachine"@en .

:ExtensionMeasuringSystem
        rdf:type        skos:Concept , owl:Class ;
        rdfs:comment    "Measuring system for measurement of extension in the area of the gauge length"@en ;
        rdfs:label      "ExtensionMeasuringSystem"@en ;
        skos:altlabel   "Extension measurement system"@en , "Dehnung"@de ;
        skos:preflabel  "ExtensionMeasuringSystem"@en .

:OriginalGaugeLength  rdf:type  skos:Concept , owl:Class ;
        rdfs:comment    "The intial gauge length given by the specimen geometry"@en , "Anfangsmesslänge "@de , "Länge zwischen den Marken zur Kennzeichnung der Messlänge (3.1) auf der Probe, die vor dem Versuch bei Raumtemperatur gemessen wird"@de ;
        rdfs:label      "OriginalGaugeLength"@en ;
        skos:altlabel   "Messlänge Lo"@de , "Messlänge Standardweg"@de , "Initial measuring length"@en , "original gauge length"@en , "Original gauge length "@en ;
        skos:preflabel  "OriginalGaugeLength"@en .

:sequence  rdf:type     owl:DatatypeProperty ;
        rdfs:domain     :Workflow ;
        rdfs:label      "sequence"@en ;
        dc:description  "The sequence of steps"@en ;
        skos:preflabel  "sequence"@en .

:FluidSolidTransition
        rdf:type        owl:Class ;
        rdfs:label      "Fluid solid transition"@en ;
        skos:preflabel  "Fluid solid transition"@en .

:RelativeStandardDeviationOfTheSlope
        rdf:type        skos:Concept , owl:Class ;
        rdfs:label      "RelativeStandardDeviationOfTheSlope"@en ;
        skos:altlabel   "relative standard deviation of the slope"@en ;
        skos:preflabel  "RelativeStandardDeviationOfTheSlope"@en .

:PercentageYieldPointExtension
        rdf:type        skos:Concept , owl:Class ;
        rdfs:label      "PercentageYieldPointExtension"@en ;
        skos:altlabel   "percentage yield point extension"@en ;
        skos:preflabel  "PercentageYieldPointExtension"@en .

:CodeFileRessource  rdf:type  owl:Class ;
        rdfs:comment     "file input or output of a job"@en ;
        rdfs:label       "File"@en , "Datei"@de ;
        rdfs:subClassOf  :CodeRessource ;
        skos:preflabel   "File"@en , "Datei"@de .

:MaterialInstabilityStrain
        rdf:type           skos:Concept , owl:Class ;
        rdfs:comment       "Critical plastic strain (material instability)\nLT.0.0: |ECRIT| is either a load curve ID defining critical equivalent plastic strain versus triaxiality or a table ID defining critical equivalent plastic strain as a function of triaxiality and Lode parameter (as in LCSDG). With HISVN ≠ 0, a 3D table can be used, where critical strain is a function of the history variable (TABLE_3D), Lode parameter (TABLE), and triaxiality (CURVE). With HISVN = 0, a 3D table introduces thermal effects, that is, critical strain is a function of temperature (TABLE_3D), Lode parameter (TABLE), and triaxiality (CURVE).\nEQ.0.0: Fixed value DCRIT defining critical damage is read (see below).\nGT.0.0: Fixed value for stress-state independent critical equivalent plastic strain."@en ;
        rdfs:label         "MaterialInstabilityStrain"@en ;
        rdfs:subClassOf    "https://material-digital.de/pmdco/ValueObject" ;
        skos:altlabel      "ECRIT"@en ;
        skos:preflabel     "MaterialInstabilityStrain"@en ;
        :UnitLabel         "-" ;
        :hasLabelSourceEn  "LS-DYNA_Manual_Volume_2" .

:YieldStress  rdf:type     skos:Concept , owl:Class ;
        rdfs:comment       "Initial yield stress, if noidentifier for hardening curve (LCSS>0) is prescibed"@en ;
        rdfs:label         "YieldStress"@en , "Yield Stress"@en , "Fließspannung"@de ;
        rdfs:subClassOf    "https://material-digital.de/pmdco/ValueObject" ;
        skos:altlabel      "SIGY"@en ;
        skos:preflabel     "Yield Stress"@en , "Fließspannung"@de , "YieldStress"@en ;
        :UnitLabel         "MPa" ;
        :hasLabelSourceEn  "LS-DYNA_Manual_Volume_2" .

:MaterialCard  rdf:type  owl:Class ;
        rdfs:comment    "The MaterialCard is a digital representation of a real world steel; for example HCT980X. It contains all information to reproduce the behaviour steel within a simulation as close as possible to it's real world counter part."@en ;
        rdfs:label      "Material Karte"@de , "Material Card"@en ;
        skos:altlabel   "Digitale Werkstoffbeschreibung"@de ;
        skos:preflabel  "Material Karte"@de , "Material Card"@en .

:FlatRolling  rdf:type  owl:Class ;
        rdfs:label      "flat rolling"@en , "Flachwalzen"@de ;
        skos:preflabel  "flat rolling"@en , "Flachwalzen"@de .

:CrashTest  rdf:type    owl:Class ;
        rdfs:label      "Crash Test"@en , "Crash Test"@de ;
        skos:preflabel  "Crash Test"@en , "Crash Test"@de .

:environment  rdf:type  owl:DatatypeProperty ;
        rdfs:domain     :Workflow ;
        rdfs:label      "environment"@en ;
        skos:preflabel  "environment"@en .

:PyironProject  rdf:type  owl:Class ;
        rdfs:comment    "A frame where all pyiron jobs are done on top of this frame. It encloses a number of jobs. It also provides utility functions for creatig python objects for these jobs."@en ;
        rdfs:label      "Pyiron project"@en , "Pyiron Projekt"@de ;
        skos:preflabel  "Pyiron project"@en , "Pyiron Projekt"@de .

:hasStrainRateFormulationFlag
        rdf:type        owl:ObjectProperty ;
        rdfs:label      "hasStrainRateFormulationFlag"@en ;
        rdfs:range      "https://w3id.org/steel/ProcessOntology/StrainRateFormulationFlag" ;
        skos:preflabel  "hasStrainRateFormulationFlag"@en .

:hasFailureStrainIdentifier4Temperature
        rdf:type        owl:ObjectProperty ;
        rdfs:label      "hasFailureStrainIdentifier4Temperature"@en ;
        rdfs:range      "https://w3id.org/steel/ProcessOntology/FailureStrainIdentifier4Temperature" ;
        skos:preflabel  "hasFailureStrainIdentifier4Temperature"@en .

:TangentYieldModulus  rdf:type  skos:Concept , owl:Class ;
        rdfs:comment       "Slope of linear hardening, if noidentifier for hardening curve (LCSS>0) is prescibed"@en ;
        rdfs:label         "TangentYieldModulus"@en ;
        rdfs:subClassOf    "https://material-digital.de/pmdco/ValueObject" ;
        skos:altlabel      "ETAN"@en ;
        skos:preflabel     "TangentYieldModulus"@en ;
        :UnitLabel         "MPa" ;
        :hasLabelSourceEn  "LS-DYNA_Manual_Volume_2" .

:hasNumberFailedIntegrationPoints
        rdf:type        owl:ObjectProperty ;
        rdfs:label      "hasNumberFailedIntegrationPoints"@en ;
        rdfs:range      "https://w3id.org/steel/ProcessOntology/NumberFailedIntegrationPoints" ;
        skos:preflabel  "hasNumberFailedIntegrationPoints"@en .

:hasFailureCriteriaTypeAdd4ElementDeletion
        rdf:type        owl:ObjectProperty ;
        rdfs:label      "hasFailureCriteriaTypeAdd4ElementDeletion"@en ;
        rdfs:range      "https://w3id.org/steel/ProcessOntology/FailureCriteriaTypeAdd4ElementDeletion" ;
        skos:preflabel  "hasFailureCriteriaTypeAdd4ElementDeletion"@en .

:Grain  rdf:type        owl:Class ;
        rdfs:label      "Korn"@de , "Grain"@en ;
        skos:preflabel  "Korn"@de , "Grain"@en .

:RollingMill  rdf:type  owl:Class ;
        rdfs:label      "rolling mill"@en , "Walzstraße"@de ;
        skos:preflabel  "rolling mill"@en , "Walzstraße"@de .

:DisplacementTransducer
        rdf:type        skos:Concept , owl:Class ;
        rdfs:comment    "Dehnungsaufnehmers (Extensometer)"@de , "Type of the displacement transducer."@en ;
        rdfs:label      "DisplacementTransducer"@en ;
        skos:altlabel   "extensometer system"@en , "Displacement transducer"@en , "Dehnungsaufnehmer"@de , "Wegaufnehmer"@de ;
        skos:preflabel  "DisplacementTransducer"@en .

:EstimatedStrainRateOverTheParallelLength
        rdf:type        skos:Concept , owl:Class ;
        rdfs:label      "EstimatedStrainRateOverTheParallelLength"@en ;
        skos:altlabel   "estimated strain rate over the parallel length"@en ;
        skos:preflabel  "EstimatedStrainRateOverTheParallelLength"@en .

:hasProjectName  rdf:type  owl:ObjectProperty ;
        rdfs:domain     :Test ;
        rdfs:label      "has project name"@en ;
        rdfs:range      :ProjectName ;
        skos:preflabel  "has project name"@en .

:Deformation  rdf:type  owl:Class ;
        rdfs:label      "Verfomung"@de , "Deformation"@en ;
        skos:preflabel  "Verfomung"@de , "Deformation"@en .

:MorphologicalTexture
        rdf:type        owl:Class ;
        rdfs:label      "Morphologische Beschaffenheit"@de , "Morphological Texture"@en ;
        skos:preflabel  "Morphologische Beschaffenheit"@de , "Morphological Texture"@en .

:FailureCriteriaTypeAdd4StrainAverage
        rdf:type           skos:Concept , owl:Class ;
        rdfs:comment       "Number of time steps for running average of plastic failure strain in the additional failure criterion"@en ;
        rdfs:label         "FailureCriteriaTypeAdd4StrainAverage"@en ;
        rdfs:subClassOf    "https://material-digital.de/pmdco/ValueObject" ;
        skos:altlabel      "NUMAVG"@en ;
        skos:preflabel     "FailureCriteriaTypeAdd4StrainAverage"@en ;
        :UnitLabel         "1" ;
        :hasLabelSourceEn  "LS-DYNA_Manual_Volume_2" .

:PhaseBoundary  rdf:type  owl:Class ;
        rdfs:label      "Phasengrenze"@de , "Phase Boundary"@en ;
        skos:preflabel  "Phasengrenze"@de , "Phase Boundary"@en .

:contactLength  rdf:type  owl:Class ;
        rdfs:label      "gedrückte Länge"@de , "contact length"@en ;
        skos:preflabel  "gedrückte Länge"@de , "contact length"@en .

:WidthStrain  rdf:type  skos:Concept , owl:Class ;
        rdfs:comment    "engineering strain in width direction"@en ;
        rdfs:label      "WidthStrain"@en ;
        skos:altlabel   "eps-Breite"@de , "engineering width strain"@en ;
        skos:preflabel  "WidthStrain"@en .

:SheetThickness  rdf:type  owl:Class ;
        rdfs:label      "Sheet thickness"@en , "Blechstärke"@de ;
        skos:altlabel   "Blechdicke"@de ;
        skos:preflabel  "Sheet thickness"@en , "Blechstärke"@de .

:Width  rdf:type        skos:Concept , owl:Class ;
        rdfs:comment    "width of the extensometer gauge length in thickness direction"@en ;
        rdfs:label      "Width"@en ;
        skos:altlabel   "Width"@en , "Breite, B"@de ;
        skos:preflabel  "Width"@en .

:StrainRateScaleIdendifier
        rdf:type           skos:Concept , owl:Class ;
        rdfs:comment       "Load curve Identifier defining strain rate scaling effect on yield stress."@en ;
        rdfs:label         "StrainRateScaleIdendifier"@en ;
        rdfs:subClassOf    "https://material-digital.de/pmdco/ValueObject" ;
        skos:altlabel      "LCSR"@en ;
        skos:preflabel     "StrainRateScaleIdendifier"@en ;
        :UnitLabel         "-" ;
        :hasLabelSourceEn  "LS-DYNA_Manual_Volume_2" .

:TestTemperature  rdf:type  owl:Class , skos:Concept ;
        rdfs:comment    "The temperature during the experiment."@en , "The initial test temperature during the experiment (neglecting adiabatic heating)"@en ;
        rdfs:label      "TestTemperature"@en ;
        skos:altlabel   "Temperature"@en , "Test temperature"@en , "Temperatur"@de , "Prüftemperatur"@de ;
        skos:preflabel  "TestTemperature"@en .

:hasTestProperty  rdf:type  owl:ObjectProperty ;
        rdfs:domain     :Test ;
        rdfs:label      "has test property"@en ;
        dc:description  "super property for all test properties"@en ;
        skos:preflabel  "has test property"@en .

:rollingSpeed  rdf:type  owl:Class ;
        rdfs:label      "rolling speed"@en , "Walzgeschwindigkeit"@de ;
        skos:altlabel   "circunferencal speed"@en , "Walzenumfangsgeschwindigleit"@de ;
        skos:preflabel  "rolling speed"@en , "Walzgeschwindigkeit"@de .

:DigitalWorkflow  rdf:type  owl:Class ;
        rdfs:comment     "Definition in the Workflow Group: \"A workflow is a chain of well-documented process steps to create or handle data for a specific problem in order to deliver a particular set of outputs.\"\nor\n\"chain of steps\""@en ;
        rdfs:label       "Digitaler Arbeitsablauf"@de , "Digital workflow"@en ;
        rdfs:subClassOf  :Workflow ;
        skos:preflabel   "Digitaler Arbeitsablauf"@de , "Digital workflow"@en .

:MatTabulatedJohnsonCookLogInterpolation
        rdf:type           skos:Concept , owl:Class ;
        rdfs:comment       "Simple incompressible plasticity model with adiabatic approach and logarithmic interpolation"@en ;
        rdfs:label         "MatTabulatedJohnsonCookLogInterpolation"@en ;
        rdfs:subClassOf    "https://material-digital.de/pmdco/ValueObject" ;
        skos:altlabel      "Mat224LogInter"@en ;
        skos:preflabel     "MatTabulatedJohnsonCookLogInterpolation"@en ;
        :hasLabelSourceEn  "LS-DYNA_Manual_Volume_2" .

:hasYieldStress  rdf:type  owl:ObjectProperty ;
        rdfs:label      "hasYieldStress"@en ;
        rdfs:range      "https://w3id.org/steel/ProcessOntology/YieldStress" ;
        skos:preflabel  "hasYieldStress"@en .

:Abaqus  rdf:type        owl:Class ;
        rdfs:comment     "Simulation Software named Abaqus"@en ;
        rdfs:label       "Abaqus"@en , "Abaqus"@de ;
        rdfs:subClassOf  :Solver ;
        skos:preflabel   "Abaqus"@en , "Abaqus"@de .

:draught  rdf:type      owl:Class ;
        rdfs:label      "draught"@en , "Höhenabnahme pro Stich"@de ;
        skos:altlabel   "height reduction"@en , "Stichabnahme"@de ;
        skos:preflabel  "draught"@en , "Höhenabnahme pro Stich"@de .

:numberOfPasses  rdf:type  owl:Class ;
        rdfs:label      "number of passes"@en , "Stichzahl"@de ;
        skos:preflabel  "number of passes"@en , "Stichzahl"@de .

:Strip  rdf:type        owl:Class ;
        rdfs:label      "strip"@en , "Band"@de ;
        skos:preflabel  "strip"@en , "Band"@de .

:Operator  rdf:type     owl:Class ;
        rdfs:comment    "some kind of a step. mathematical Operator"@en ;
        rdfs:label      "Operator"@en , "Mathematische Operation"@de ;
        skos:preflabel  "Operator"@en , "Mathematische Operation"@de .

:WidthChange  rdf:type  skos:Concept , owl:Class ;
        rdfs:comment    "change of width of the extensometer gauge length"@en , "Change of the sample width."@en ;
        rdfs:label      "WidthChange"@en ;
        skos:altlabel   "dB"@de , "Width change"@en , "Breitenänderung"@de ;
        skos:preflabel  "WidthChange"@en .

:ShearLength  rdf:type  skos:Concept , owl:Class ;
        rdfs:comment    "length of the shear zone"@en , "Länge der Scherzone"@de ;
        rdfs:label      "ShearLength"@en ;
        skos:altlabel   "ShearLength"@en ;
        skos:preflabel  "ShearLength"@en .

:MegaPA-PER-SEC  rdf:type  owl:Class ;
        rdfs:comment    "Stress rate, e.g. referenced by tensile tests"@en ;
        rdfs:label      "Mega Pascal pro Sekunde"@de , "Mega Pascal per Second"@en ;
        rdfs:seeAlso    <qudt:MegaPA> ;
        skos:preflabel  "Mega Pascal pro Sekunde"@de , "Mega Pascal per Second"@en ;
        skos:related    <qudt:MegaPA> .

:FractureStrain  rdf:type  owl:Class ;
        rdfs:label      "Fracture Strain"@en , "Bruchdehnung"@de ;
        skos:preflabel  "Fracture Strain"@en , "Bruchdehnung"@de .

:InitialDisplacementRate
        rdf:type        skos:Concept , owl:Class ;
        rdfs:comment    "The velocity of the actuator"@en ;
        rdfs:label      "InitialDisplacementRate"@en ;
        skos:altlabel   "Initial displacement rate v0"@en , "Abzugsgeschw."@de ;
        skos:preflabel  "InitialDisplacementRate"@en .

:FailureStrain  rdf:type   skos:Concept , owl:Class ;
        rdfs:comment       "Failure strain curve/table or function\nGT.0.0: Load curve ID or table ID. As a load curve, it defines equivalent plastic strain to failure as a function of triaxiality. As a table, it defines for each Lode parameter value (between -1 and 1) a load curve ID giving the\nequivalent plastic strain to failure as a function of triaxiality for that Lode parameter value. With HISVN ≠ 0, a 3D table can be used, where failure strain is a function of the history variable (TABLE_3D), Lode parameter (TABLE), and triaxiality (CURVE). With HISVN = 0, a 3D table introduces thermal effects, that is, failure strain is a function of temperature (TABLE_3D), Lode parameter (TABLE), and triaxiality (CURVE).\nLT.0.0: |LCSDG| is the ID of a function (*DEFINE_FUNCTION) with the arguments triaxiality and Lode parameter: 𝑓 (𝜂, 𝐿)."@en ;
        rdfs:label         "FailureStrain"@en ;
        rdfs:subClassOf    "https://material-digital.de/pmdco/ValueObject" ;
        skos:altlabel      "LCSDG"@en ;
        skos:preflabel     "FailureStrain"@en ;
        :UnitLabel         "-" ;
        :hasLabelSourceEn  "LS-DYNA_Manual_Volume_2" .

:SampleIdentifier-2  rdf:type  skos:Concept , owl:Class ;
        rdfs:comment    "Unique ID (IWM intern)"@en ;
        rdfs:label      "SampleIdentifier-2"@en ;
        skos:altlabel   "Sample identifier 2"@en , "Probenkennung 2"@de ;
        skos:preflabel  "SampleIdentifier-2"@en .

:transverseDirection  rdf:type  owl:Class ;
        rdfs:label      "transverse direction"@en , "Querrichtung"@de ;
        skos:altlabel   "TD"@en ;
        skos:preflabel  "transverse direction"@en , "Querrichtung"@de .

:SampleCode  rdf:type   skos:Concept , owl:Class ;
        rdfs:label      "SampleCode"@en ;
        skos:altlabel   "QR-Code from Label System"@en , "QR-Code"@de ;
        skos:preflabel  "SampleCode"@en .

:InitialThickness  rdf:type  owl:Class ;
        rdfs:label      "initial thickness"@en , "Anfangsdicke"@de ;
        skos:preflabel  "initial thickness"@en , "Anfangsdicke"@de .

:PercentageTotalExtensionAtMaximumForce
        rdf:type        skos:Concept , owl:Class ;
        rdfs:label      "PercentageTotalExtensionAtMaximumForce"@en ;
        skos:altlabel   "percentage total extension at maximum force"@en ;
        skos:preflabel  "PercentageTotalExtensionAtMaximumForce"@en .

:ThicknessAfterFracture1
        rdf:type        skos:Concept , owl:Class ;
        rdfs:label      "ThicknessAfterFracture1"@en ;
        skos:altlabel   "Thickness A1 after fracture"@en , "Probendicke A1 nach Bruch"@de ;
        skos:preflabel  "ThicknessAfterFracture1"@en .

:Standard  rdf:type     owl:Class ;
        rdfs:comment    "Standard as described by ISO / DIN / etc"@en ;
        rdfs:label      "Standard"@en , "Norm"@de ;
        skos:preflabel  "Standard"@en , "Norm"@de .

:SimulationCode  rdf:type  owl:Class ;
        rdfs:label       "Simulations Code"@de , "Simulation Code"@en ;
        rdfs:subClassOf  :Code ;
        skos:altlabel    "Simulationsprogramm"@de , "Simulation program"@en ;
        skos:preflabel   "Simulations Code"@de , "Simulation Code"@en .

:MaximumForceNoDiscontinousYielding
        rdf:type        skos:Concept , owl:Class ;
        rdfs:label      "MaximumForceNoDiscontinousYielding"@en ;
        skos:altlabel   "maximum force \"no discontinous yielding\""@en ;
        skos:preflabel  "MaximumForceNoDiscontinousYielding"@en .

:Benchmark  rdf:type    owl:Class ;
        rdfs:label      "Messlatte"@de , "Benchmark"@en ;
        skos:altlabel   "Richtwert"@de , " Maßstab"@de , " Bezugspunkt"@de ;
        skos:preflabel  "Messlatte"@de , "Benchmark"@en .

:FrameOfMaterial  rdf:type  owl:Class ;
        rdfs:label      "frame of material"@en , "Rahmenmaterial"@de ;
        skos:preflabel  "frame of material"@en , "Rahmenmaterial"@de .

:OriginalWidth  rdf:type  owl:Class , skos:Concept ;
        rdfs:comment    "The width of the specimen."@en , "Original width of the parallel length of a flat test piece"@en ;
        rdfs:label      "OriginalWidth"@en ;
        skos:altlabel   "Probenbreite b"@de , "Specimen width"@en , "Probenbreite"@de , "Probenbreite b0"@de , "Original width"@en ;
        skos:preflabel  "OriginalWidth"@en .

:hasHDF  rdf:type       owl:ObjectProperty ;
        rdfs:domain     :PyironJob ;
        rdfs:label      "has hdf"@en ;
        rdfs:range      :HDF5 ;
        dc:description  "The pyiron jobs has hdf5 file"@en ;
        skos:preflabel  "has hdf"@en .

:hasSubJob  rdf:type    owl:ObjectProperty ;
        rdfs:domain     :PyironJob ;
        rdfs:label      "has a sub job"@en ;
        rdfs:range      :PyironJob ;
        skos:preflabel  "has a sub job"@en .

:OriginalThickness  rdf:type  owl:Class , skos:Concept ;
        rdfs:comment    "Original width of the parallel length of a flat test piece"@en , "The thickness of the specimen."@en , "The initial thickness of the specimen."@en ;
        rdfs:label      "OriginalThickness"@en ;
        skos:altlabel   "Probendicke a"@de , "Specimen thickness"@en , "Probendicke a0"@de , "Original thickness"@en , "Probendicke"@de ;
        skos:preflabel  "OriginalThickness"@en .

:FadingExponent  rdf:type  skos:Concept , owl:Class ;
        rdfs:comment       "Exponent for damage-related stress fadeout:\nLT.0.0: |FADEXP| is a load curve ID defining element-size dependent fading exponent.\nGT.0.0: Constant fading exponent"@en ;
        rdfs:label         "FadingExponent"@en ;
        rdfs:subClassOf    "https://material-digital.de/pmdco/ValueObject" ;
        skos:altlabel      "FADEXP"@en ;
        skos:preflabel     "FadingExponent"@en ;
        :UnitLabel         "1" ;
        :hasLabelSourceEn  "LS-DYNA_Manual_Volume_2" .

:hasStrainRateScaleParameterP
        rdf:type        owl:ObjectProperty ;
        rdfs:label      "hasStrainRateScaleParameterP"@en ;
        rdfs:range      "https://w3id.org/steel/ProcessOntology/StrainRateScaleParameterP" ;
        skos:preflabel  "hasStrainRateScaleParameterP"@en .

:PyironJob  rdf:type     owl:Class ;
        rdfs:comment     "execution information of a Code; can get deferred; can get executed on a batch system. A Pyiron job bundles all required metadata for a Pyiron code execution. Is similar to the context of a process from computer science."@en ;
        rdfs:label       "Pyiron Job"@en , "Pyiron Job"@de ;
        rdfs:subClassOf  emmo:process ;
        skos:altlabel    " Pyiron execution context"@en , " Pyiron Kontext"@de , " Pyiron Prozess"@de , "Pyiron Job"@de , "Pyiron process"@en ;
        skos:preflabel   "Pyiron Job"@en , "Pyiron Job"@de .

:Code   rdf:type        owl:Class ;
        rdfs:comment    "A external general simulation program. e.g. DAMASK or LAMMPS. A Code gets executed by a job"@en ;
        rdfs:label      "Code"@en , "Code"@de ;
        rdfs:seeAlso    :Software ;
        skos:altlabel   "Ablauf"@de ;
        skos:preflabel  "Code"@en , "Code"@de ;
        skos:related    :Software .

:PercentageExtension  rdf:type  skos:Concept , owl:Class ;
        rdfs:comment    "engineering strain"@en ;
        rdfs:label      "PercentageExtension"@en ;
        skos:altlabel   "percentage extension"@en , "eps-technisch"@de , "e-technisch"@de , "Time-dependent engineering strain"@en ;
        skos:preflabel  "PercentageExtension"@en .

:Radius  rdf:type       skos:Concept , owl:Class ;
        rdfs:comment    "Radius of the notch (only for notched shear tensile specimens)"@en , "Kerbradius (nur bei Schrägkerb-Scherzugproben)"@de ;
        rdfs:label      "Radius"@en ;
        skos:altlabel   "Radius"@en ;
        skos:preflabel  "Radius"@en .

:hasDamageExponent  rdf:type  owl:ObjectProperty ;
        rdfs:label      "hasDamageExponent"@en ;
        rdfs:range      "https://w3id.org/steel/ProcessOntology/DamageExponent" ;
        skos:preflabel  "hasDamageExponent"@en .

:CrystallographyTexture
        rdf:type        owl:Class ;
        rdfs:label      "Kristallographische Beschaffenheit"@de , "Crystollography Texture"@en ;
        skos:preflabel  "Kristallographische Beschaffenheit"@de , "Crystollography Texture"@en .

:hasInput  rdf:type     owl:ObjectProperty ;
        rdfs:domain     :Code ;
        rdfs:label      "has input"@en ;
        rdfs:range      :CodeRessource ;
        dc:description  "input ressource for a Code"@en ;
        skos:preflabel  "has input"@en .

:TruePlasticStrainAtFracture
        rdf:type        skos:Concept , owl:Class ;
        rdfs:comment    "true plastic strain at fracture"@en ;
        rdfs:label      "TruePlasticStrainAtFracture"@en ;
        skos:altlabel   "wahre Bruchdehnung"@de , "True plastic strain at fracture"@en ;
        skos:preflabel  "TruePlasticStrainAtFracture"@en .

:DamageTreatment  rdf:type  skos:Concept , owl:Class ;
        rdfs:comment       "interpreted digit-wise as follows: DTYP = [𝑁𝑀] = 𝑀+10×𝑁\nM.EQ.0: Damage is accumulated, but there is no coupling to flow stress and no failure.\nM.EQ.1: Damage is accumulated, and element failure occurs for 𝐷 = 1. Coupling of damage to flow stress depending on parameters.\nN.EQ.0: Equivalent plastic strain is the driving quantity for the damage.\nN.GT.0: The Nth additional history variable is the driving quantity for damage."@en ;
        rdfs:label         "DamageTreatment"@en ;
        rdfs:subClassOf    "https://material-digital.de/pmdco/ValueObject" ;
        skos:altlabel      "DTYP"@en ;
        skos:preflabel     "DamageTreatment"@en ;
        :UnitLabel         "1" ;
        :hasLabelSourceEn  "LS-DYNA_Manual_Volume_2" .

:JobInput  rdf:type      owl:Class ;
        rdfs:comment     "the input parameter for a pyiron job"@en ;
        rdfs:label       "Pyiron job input"@en , "Job-Input-Parameter"@de ;
        rdfs:seeAlso     :PyironJob ;
        rdfs:subClassOf  :CodeRessource ;
        skos:preflabel   "Pyiron job input"@en , "Job-Input-Parameter"@de ;
        skos:related     :PyironJob .

:SimulationWorkflow  rdf:type  owl:Class ;
        rdfs:label       "Simulationsablauf"@de , "Simulation Workflow"@en ;
        rdfs:subClassOf  :Workflow ;
        skos:preflabel   "Simulationsablauf"@de , "Simulation Workflow"@en .

:CodeRessource  rdf:type  owl:Class ;
        rdfs:comment    "Input or output of a job"@en ;
        rdfs:label      "Resource"@en ;
        skos:preflabel  "Resource"@en .

:FeedbackLoop  rdf:type  owl:Class ;
        rdfs:label      "Rückkopplung"@de , "Feedback Loop"@en ;
        skos:preflabel  "Rückkopplung"@de , "Feedback Loop"@en .

:TimeDependentEngineeringStrainRate
        rdf:type        skos:Concept , owl:Class ;
        rdfs:label      "TimeDependentEngineeringStrainRate"@en ;
        skos:altlabel   "Time-dependent engineering strain rate"@en , "Dehnrate"@de ;
        skos:preflabel  "TimeDependentEngineeringStrainRate"@en .

<https://w3id.org/steel/ProcessOntology/ProofStrength%2CPlasticExtension>
        rdf:type        skos:Concept , owl:Class ;
        rdfs:label      "ProofStrength,PlasticExtension"@en ;
        skos:altlabel   "proof strength, plastic extension"@en ;
        skos:preflabel  "ProofStrength,PlasticExtension"@en .

:hasProjectNumber  rdf:type  owl:ObjectProperty ;
        rdfs:domain     :Test ;
        rdfs:label      "has project number"@en ;
        rdfs:range      :ProjectNumber ;
        skos:preflabel  "has project number"@en .

:PermanentSetStrength
        rdf:type        skos:Concept , owl:Class ;
        rdfs:label      "PermanentSetStrength"@en ;
        skos:altlabel   "permanent set strength"@en ;
        skos:preflabel  "PermanentSetStrength"@en .

:hasTestingFacility  rdf:type  owl:ObjectProperty ;
        rdfs:domain     :Test ;
        rdfs:label      "has testing facility"@en ;
        rdfs:range      :TestingFacility ;
        skos:preflabel  "has testing facility"@en .

:MatPiecewiseLinearPlasticityLogInterpolation
        rdf:type           skos:Concept , owl:Class ;
        rdfs:comment       "Simple incompressible plasticity model with logarithmic interpolation"@en ;
        rdfs:label         "MatPiecewiseLinearPlasticityLogInterpolation"@en ;
        rdfs:subClassOf    "https://material-digital.de/pmdco/ValueObject" ;
        skos:altlabel      "Mat024LogInter"@en ;
        skos:preflabel     "MatPiecewiseLinearPlasticityLogInterpolation"@en ;
        :hasLabelSourceEn  "LS-DYNA_Manual_Volume_2" .

:DataSamplingFrequency
        rdf:type        skos:Concept , owl:Class ;
        rdfs:comment    "Die Frequenz-Bandweite jedes Messkanals sowie die Messwerterfassungsfrequenz sollten ausreichend hoch sein, damit die zu bestimmenden Werkstoffkenngrößen aufgezeichnet werden können. So kann z. B. bei Ermittlung von ReH die Gleichung (A.1) zur Bestimmung der in 1/Sekunde angegebenen Mindestmesswert-erfassungsgrenze fmin verwendet werden:"@de ;
        rdfs:label      "DataSamplingFrequency"@en ;
        skos:altlabel   "Data sampling frequency"@en ;
        skos:preflabel  "DataSamplingFrequency"@en .

:hasMinTimeStep4ElementDel
        rdf:type        owl:ObjectProperty ;
        rdfs:label      "hasMinTimeStep4ElementDel"@en ;
        rdfs:range      "https://w3id.org/steel/ProcessOntology/MinTimeStep4ElementDel" ;
        skos:preflabel  "hasMinTimeStep4ElementDel"@en .

:ForceAtFracture  rdf:type  skos:Concept , owl:Class ;
        rdfs:label      "ForceAtFracture"@en ;
        skos:preflabel  "ForceAtFracture"@en .

:TensileTest  rdf:type  owl:Class ;
        rdfs:label      "Zugversuch"@de , "Tensile Test"@en ;
        rdfs:seeAlso    pmdco:TensileTest ;
        skos:preflabel  "Zugversuch"@de , "Tensile Test"@en ;
        skos:related    pmdco:TensileTest .

:UltimateTensileStrength
        rdf:type        owl:Class ;
        rdfs:label      "Zugfestigkeit"@de , "Ultimate Tensile Strength"@en ;
        skos:preflabel  "Zugfestigkeit"@de , "Ultimate Tensile Strength"@en .

:Test   rdf:type        owl:Class ;
        rdfs:comment    "like Tensile Test etc, maybe an experiment"@en ;
        rdfs:label      "Test"@en , "Test"@de ;
        skos:preflabel  "Test"@en , "Test"@de .

:ExperimentalWorkflow
        rdf:type         owl:Class ;
        rdfs:label       "Experimenteller Arbeitsablauf"@de , "Experimental workflow"@en ;
        rdfs:subClassOf  :Workflow ;
        skos:preflabel   "Experimenteller Arbeitsablauf"@de , "Experimental workflow"@en .

:MatPiecewiseLinearPlasticity
        rdf:type           skos:Concept , owl:Class ;
        rdfs:comment       "Simple incompressible plasticity model"@en ;
        rdfs:label         "MatPiecewiseLinearPlasticity"@en ;
        rdfs:subClassOf    "https://material-digital.de/pmdco/ValueObject" ;
        skos:altlabel      "Mat024"@en ;
        skos:preflabel     "MatPiecewiseLinearPlasticity"@en ;
        :hasLabelSourceEn  "LS-DYNA_Manual_Volume_2" .

:ElementDeletionFlag  rdf:type  skos:Concept , owl:Class ;
        rdfs:comment       "Erosion flag (only for solid elements):\n=0.0: default, element erosion is allowed\n=1.0: element does not erode; deviatoric stresses set to 0 when element fails"@en ;
        rdfs:label         "ElementDeletionFlag"@en ;
        rdfs:subClassOf    "https://material-digital.de/pmdco/ValueObject" ;
        skos:altlabel      "ERODE"@en ;
        skos:preflabel     "ElementDeletionFlag"@en ;
        :UnitLabel         "-" ;
        :hasLabelSourceEn  "LS-DYNA_Manual_Volume_2" .

:PercentageElongation
        rdf:type        skos:Concept , owl:Class ;
        rdfs:comment    "Verlängerung (3.3), angegeben in Prozent, bezogen auf die Anfangsmesslänge (3.1.1)"@de ;
        rdfs:label      "PercentageElongation"@en ;
        skos:altlabel   "percentage elongation"@en , "Elongation"@en , "Dehnung"@de ;
        skos:preflabel  "PercentageElongation"@en .

:hasMAT_ADD_DAMAGE_GISSMO
        rdf:type        owl:ObjectProperty ;
        rdfs:label      "hasMAT_ADD_DAMAGE_GISSMO"@en ;
        rdfs:range      "https://w3id.org/steel/ProcessOntology/MAT_ADD_DAMAGE_GISSMO" ;
        skos:preflabel  "hasMAT_ADD_DAMAGE_GISSMO"@en .

:hasMatTabulatedJohnsonCookLogInterpolation
        rdf:type        owl:ObjectProperty ;
        rdfs:label      "hasMatTabulatedJohnsonCookLogInterpolation"@en ;
        rdfs:range      "https://w3id.org/steel/ProcessOntology/MatTabulatedJohnsonCookLogInterpolation" ;
        skos:preflabel  "hasMatTabulatedJohnsonCookLogInterpolation"@en .

:PercentageElongationAfterFracture
        rdf:type        owl:Class , skos:Concept ;
        rdfs:comment    "bleibende Verlängerung (3.3) der Messlänge nach dem Bruch (Lu − Lo), angegeben in Prozent, bezogen auf die Anfangsmesslänge (3.1.1)"@de , "percentage elongation after fracture"@en ;
        rdfs:label      "PercentageElongationAfterFracture"@en ;
        skos:altlabel   "Bruchdehnung A_20mm"@de , "Bruchdehnung A20mm"@de , "A"@de , "percentage elongation after fracture"@en ;
        skos:preflabel  "PercentageElongationAfterFracture"@en .

:hasYieldingIdentifierIsoThermal
        rdf:type        owl:ObjectProperty ;
        rdfs:label      "hasYieldingIdentifierIsoThermal"@en ;
        rdfs:range      "https://w3id.org/steel/ProcessOntology/YieldingIdentifierIsoThermal" ;
        skos:preflabel  "hasYieldingIdentifierIsoThermal"@en .

:StandardDeviationOfTheSlope
        rdf:type        skos:Concept , owl:Class ;
        rdfs:label      "StandardDeviationOfTheSlope"@en ;
        skos:altlabel   "standard deviation of the slope"@en ;
        skos:preflabel  "StandardDeviationOfTheSlope"@en .

:GaugeLength  rdf:type  skos:Concept , owl:Class ;
        rdfs:comment    "Länge des parallelen Teils der Probe, an dem zu einem beliebigen Zeitpunkt während des Versuchs die Verlängerung gemessen wird"@de ;
        rdfs:label      "GaugeLength"@en ;
        skos:altlabel   "gauge length"@en ;
        skos:preflabel  "GaugeLength"@en .

:ThicknessAfterFracture2
        rdf:type        skos:Concept , owl:Class ;
        rdfs:label      "ThicknessAfterFracture2"@en ;
        skos:altlabel   "Thickness A2 after fracture"@en , "Probendicke A2 nach Bruch"@de ;
        skos:preflabel  "ThicknessAfterFracture2"@en .

:rollingSchedule  rdf:type  owl:Class ;
        rdfs:label      "rolling schedule"@en , "Stichplan"@de ;
        skos:preflabel  "rolling schedule"@en , "Stichplan"@de .

:MachineData  rdf:type  skos:Concept , owl:Class ;
        rdfs:comment    "Die Prüfmaschine sollte mit einer analogen Messwertausgabe, die nicht durch die Software beeinflusst wird, ausgerüstet sein. Ist eine solche Ausgabe nicht vorgesehen, sollten digitale Rohdaten ausgegeben werden können. Der Prüfmaschinenhersteller sollte Auskunft über die Erzeugung der digitalen Rohdaten und ihre Verarbeitung durch die Software geben. Die Rohdaten sollten in SI-Einheiten angegeben werden und sich auf die Kraft, die Verlängerung (der Extensometer-Messlänge), den Traversenweg, die Zeit und die Probenmaße beziehen. Ein Beispiel eines geeigneten Datenformats ist in Bild A.1 dargestellt."@de ;
        rdfs:label      "MachineData"@en ;
        skos:preflabel  "MachineData"@en .

:normalDirection  rdf:type  owl:Class ;
        rdfs:label      "normal direction"@en , "Normalenrichtung"@de ;
        skos:altlabel   "ND"@en ;
        skos:preflabel  "normal direction"@en , "Normalenrichtung"@de .

:Extension  rdf:type    skos:Concept , owl:Class ;
        rdfs:comment    "Displacement of the extensometer (!) length"@en ;
        rdfs:label      "Extension"@en ;
        skos:altlabel   "Standardweg"@de , "Standard travel"@en , "extension"@en , "dL"@de , "Extension"@en ;
        skos:preflabel  "Extension"@en .

:Simulation  rdf:type   owl:Class ;
        rdfs:label      "Simulation"@en , "Simulation"@de ;
        skos:preflabel  "Simulation"@en , "Simulation"@de .

:TrueWidthStrain  rdf:type  skos:Concept , owl:Class ;
        rdfs:comment    "true strain in width direction"@en ;
        rdfs:label      "TrueWidthStrain"@en ;
        skos:altlabel   "true width strain"@en , "eps-wBreite"@de ;
        skos:preflabel  "TrueWidthStrain"@en .

:WidthAfterFracture1  rdf:type  skos:Concept , owl:Class ;
        rdfs:label      "WidthAfterFracture1"@en ;
        skos:altlabel   "Width B1 after fracture"@en , "Probenbreite B1 nach Bruch"@de ;
        skos:preflabel  "WidthAfterFracture1"@en .

:ShearTest  rdf:type    owl:Class ;
        rdfs:label      "Shear Test"@en , "Schertest"@de ;
        skos:preflabel  "Shear Test"@en , "Schertest"@de .

:YieldStrength  rdf:type  skos:Concept , owl:Class ;
        rdfs:label      "YieldStrength"@en ;
        skos:altlabel   "yield strength"@en ;
        skos:preflabel  "YieldStrength"@en .

:YieldSurface  rdf:type  owl:Class ;
        rdfs:label      "Yield surface"@en , "Ertragsfläche"@de ;
        skos:preflabel  "Yield surface"@en , "Ertragsfläche"@de .

:ExperimentalTest  rdf:type  owl:Class ;
        rdfs:comment    "Suclasses like Tensile Test"@en ;
        rdfs:label      "Experimentaler Test"@de , "Experimental test"@en ;
        skos:preflabel  "Experimentaler Test"@de , "Experimental test"@en .

:Precipitation  rdf:type  owl:Class ;
        rdfs:label      "Percipation"@en , "??"@de ;
        skos:altlabel   "Ausscheidungshärtung"@de ;
        skos:preflabel  "Percipation"@en , "??"@de .

:FailureStrainIdentifier
        rdf:type           skos:Concept , owl:Class ;
        rdfs:comment       "The load curve ID defines plastic failure strain as a function of triaxiality. The table ID defines for each Lode parameter a load curve ID giving the plastic failure strain versus triaxiality for that Lode parameter"@en ;
        rdfs:label         "FailureStrainIdentifier"@en ;
        rdfs:subClassOf    "https://material-digital.de/pmdco/ValueObject" ;
        skos:altlabel      "LCF"@en ;
        skos:preflabel     "FailureStrainIdentifier"@en ;
        :UnitLabel         "-" ;
        :hasLabelSourceEn  "LS-DYNA_Manual_Volume_2" .

:hasDamageThreshold  rdf:type  owl:ObjectProperty ;
        rdfs:label      "hasDamageThreshold"@en ;
        rdfs:range      "https://w3id.org/steel/ProcessOntology/DamageThreshold" ;
        skos:preflabel  "hasDamageThreshold"@en .

:metadata  rdf:type     owl:DatatypeProperty ;
        rdfs:domain     :Workflow ;
        rdfs:label      "metadata"@en ;
        skos:preflabel  "metadata"@en .

:JobMetadata  rdf:type  owl:Class ;
        rdfs:comment    "each pyiron job has some metadata which is stored in the central sql database"@en ;
        rdfs:label      "Pyiron job metadata"@en , "Job-Metadaten"@de ;
        skos:preflabel  "Pyiron job metadata"@en , "Job-Metadaten"@de .

:hasMatPiecewiseLinearPlasticityLogInterpolation
        rdf:type        owl:ObjectProperty ;
        rdfs:label      "hasMatPiecewiseLinearPlasticityLogInterpolation"@en ;
        rdfs:range      "https://w3id.org/steel/ProcessOntology/MatPiecewiseLinearPlasticityLogInterpolation" ;
        skos:preflabel  "hasMatPiecewiseLinearPlasticityLogInterpolation"@en .

:stripTension  rdf:type  owl:Class ;
        rdfs:label      "strip tension"@en , "Bandzug"@de ;
        skos:preflabel  "strip tension"@en , "Bandzug"@de .

:Stress  rdf:type       skos:Concept , owl:Class ;
        rdfs:label      "Stress"@en , "Spannung"@de ;
        skos:altlabel   "stress"@en ;
        skos:preflabel  "Stress"@en , "Spannung"@de .

:ConstitutiveModelParameter
        rdf:type  owl:Class .

:YoungsModulus  rdf:type   skos:Concept , owl:Class ;
        rdfs:comment       "Linear Elastic Modulus to determine the linear elasticity"@en ;
        rdfs:label         "YoungsModulus"@en ;
        rdfs:subClassOf    "https://material-digital.de/pmdco/ValueObject" ;
        skos:altlabel      "E"@en ;
        skos:preflabel     "YoungsModulus"@en ;
        :UnitLabel         "MPa" ;
        :hasLabelSourceEn  "LS-DYNA_Manual_Volume_2" .

:hasElementDeletionFlag
        rdf:type        owl:ObjectProperty ;
        rdfs:label      "hasElementDeletionFlag"@en ;
        rdfs:range      "https://w3id.org/steel/ProcessOntology/ElementDeletionFlag" ;
        skos:preflabel  "hasElementDeletionFlag"@en .

:hasMaterialInstabilityStrain
        rdf:type        owl:ObjectProperty ;
        rdfs:label      "hasMaterialInstabilityStrain"@en ;
        rdfs:range      "https://w3id.org/steel/ProcessOntology/MaterialInstabilityStrain" ;
        skos:preflabel  "hasMaterialInstabilityStrain"@en .

:CoordinateSystem  rdf:type  owl:Class ;
        rdfs:label      "Koordinatensystem"@de , "Coordinate system"@en ;
        skos:altlabel   "Koordinatensystem?"@de ;
        skos:preflabel  "Koordinatensystem"@de , "Coordinate system"@en .

:ParallelLength  rdf:type  skos:Concept , owl:Class ;
        rdfs:comment    "The length of the experiment (description replaced by Zugversuch Instron)"@en , "Länge des parallelen reduzierten Querschnitts der Probe"@de , "The length of the parallel part of the specimen"@en ;
        rdfs:label      "ParallelLength"@en ;
        skos:altlabel   "parallel length"@en , "parallele Messlänge Lc"@de , "Test length"@en , "Messlänge Lc"@de , "Parallel length"@en , "Versuchslänge"@de ;
        skos:preflabel  "ParallelLength"@en .

:hasYieldingIdentifier
        rdf:type        owl:ObjectProperty ;
        rdfs:label      "hasYieldingIdentifier"@en ;
        rdfs:range      "https://w3id.org/steel/ProcessOntology/YieldingIdentifier" ;
        skos:preflabel  "hasYieldingIdentifier"@en .

:hasSpecificHeatCapacity
        rdf:type        owl:ObjectProperty ;
        rdfs:label      "hasSpecificHeatCapacity"@en ;
        rdfs:range      "https://w3id.org/steel/ProcessOntology/SpecificHeatCapacity" ;
        skos:preflabel  "hasSpecificHeatCapacity"@en .

:FailureStrainIdentifier4StrainRate
        rdf:type           skos:Concept , owl:Class ;
        rdfs:comment       "Load curve ID defining plastic failure strain as a function of plastic strain rate"@en ;
        rdfs:label         "FailureStrainIdentifier4StrainRate"@en ;
        rdfs:subClassOf    "https://material-digital.de/pmdco/ValueObject" ;
        skos:altlabel      "LCG"@en ;
        skos:preflabel     "FailureStrainIdentifier4StrainRate"@en ;
        :UnitLabel         "-" ;
        :hasLabelSourceEn  "LS-DYNA_Manual_Volume_2" .

:ExtensionAtFracture  rdf:type  skos:Concept , owl:Class ;
        rdfs:comment    "Displacement of the extensometer (!) length at fracture"@en ;
        rdfs:label      "ExtensionAtFracture"@en ;
        skos:altlabel   "Extension at fracture"@en , "Bruchverlängerung"@de ;
        skos:preflabel  "ExtensionAtFracture"@en .

:PrincipalStressLimit4PostProcessing
        rdf:type           skos:Concept , owl:Class ;
        rdfs:comment       "Table ID with first principal stress limit as function of plastic strain (curves) and plastic strain rate (table). This option is for post-processing purposes only and gives an indication of areas in the structure where failure is likely to occur"@en ;
        rdfs:label         "PrincipalStressLimit4PostProcessing"@en ;
        rdfs:subClassOf    "https://material-digital.de/pmdco/ValueObject" ;
        skos:altlabel      "LCPS"@en ;
        skos:preflabel     "PrincipalStressLimit4PostProcessing"@en ;
        :UnitLabel         "-" ;
        :hasLabelSourceEn  "LS-DYNA_Manual_Volume_2" .

:UnusualResult  rdf:type  owl:Class ;
        rdfs:comment    "Exeriment result that differs from a given simulation result, or the other way round."@en ;
        rdfs:label      "Unusual result"@en , "Ungewöhnliches Ergebnis"@de ;
        skos:altlabel   "Unerwarteter Ausgang"@de ;
        skos:preflabel  "Unusual result"@en , "Ungewöhnliches Ergebnis"@de .

:ExperimentIdentifier
        rdf:type        skos:Concept , owl:Class ;
        rdfs:label      "ExperimentIdentifier"@en ;
        skos:altlabel   "Proben-ID"@de , "Identifier based on Label-System"@en ;
        skos:preflabel  "ExperimentIdentifier"@en .

:DamaskCode  rdf:type    owl:Class ;
        rdfs:label       "Damask code"@en , "Damask Code"@de ;
        rdfs:subClassOf  :Code ;
        skos:altlabel    "code damask"@en , "Damask Ablauf"@de ;
        skos:preflabel   "Damask code"@en , "Damask Code"@de .

:Coating  rdf:type      owl:Class ;
        rdfs:comment    "Thing that you put on the surface of a specimen that influences the surface behaviour"@en ;
        rdfs:label      "Coating"@en , "Beschichtung"@de ;
        skos:preflabel  "Coating"@en , "Beschichtung"@de .

:hasStandard  rdf:type  owl:ObjectProperty ;
        rdfs:label      "has standard"@en ;
        rdfs:range      :Standard ;
        dc:description  "the related standard (ISO / DIN / etc)"@en ;
        skos:altlabel   "has norm"@en ;
        skos:preflabel  "has standard"@en .

:WorkflowStep  rdf:type  owl:Class ;
        rdfs:comment    "a part of a workflow"@en ;
        rdfs:label      "Workflow step"@en , "Arbeitsschritt"@de ;
        skos:preflabel  "Workflow step"@en , "Arbeitsschritt"@de .

:StrainRateScaleParameterC
        rdf:type           skos:Concept , owl:Class ;
        rdfs:comment       "Parameter C for strain rate approach for using the Cowper and Symonds model which scales the yield stress with the factor: 1+(epsDot/C)^(1/P)"@en ;
        rdfs:label         "StrainRateScaleParameterC"@en ;
        rdfs:subClassOf    "https://material-digital.de/pmdco/ValueObject" ;
        skos:altlabel      "C"@en ;
        skos:preflabel     "StrainRateScaleParameterC"@en ;
        :UnitLabel         "1" ;
        :hasLabelSourceEn  "LS-DYNA_Manual_Volume_2" .

:ReferenceTemperature
        rdf:type           skos:Concept , owl:Class ;
        rdfs:comment       "Slope of linear hardening, if noidentifier for hardening curve (LCSS>0) is prescibed"@en ;
        rdfs:label         "ReferenceTemperature"@en ;
        rdfs:subClassOf    "https://material-digital.de/pmdco/ValueObject" ;
        skos:altlabel      "TR"@en ;
        skos:preflabel     "ReferenceTemperature"@en ;
        :UnitLabel         "K" ;
        :hasLabelSourceEn  "LS-DYNA_Manual_Volume_2" .

:hasFailureStrainIdentifier4MeshDependency
        rdf:type        owl:ObjectProperty ;
        rdfs:label      "hasFailureStrainIdentifier4MeshDependency"@en ;
        rdfs:range      "https://w3id.org/steel/ProcessOntology/FailureStrainIdentifier4MeshDependency" ;
        skos:preflabel  "hasFailureStrainIdentifier4MeshDependency"@en .

:PreliminaryForce  rdf:type  owl:Class , skos:Concept ;
        rdfs:comment    "Um ein Ausrichten der Probe in der Einspannvorrichtung zu erreichen, darf eine Vorkraft aufgebracht werden, die 5 % des spezifizierten oder zu erwartenden Streckgrenzenwertes nicht überschreitet. Eine Korrektur der Dehnung sollte unter Berücksichtigung der Vorkraft vorgenommen werden."@de , "\"Vorkraft\" in DIN EN ISO 6892-1"@en ;
        rdfs:label      "PreliminaryForce"@en ;
        skos:altlabel   "Vorlast"@de , "Preliminary force"@en , "PreliminaryForce"@en , "Preload"@en , "Vorkraft"@de ;
        skos:preflabel  "PreliminaryForce"@en .

:AbsoluteCrossheadTravel
        rdf:type        skos:Concept , owl:Class ;
        rdfs:comment    "Absolute position of the crosshead."@en , "Absolute position der Traverse"@de ;
        rdfs:label      "AbsoluteCrossheadTravel"@en ;
        skos:altlabel   "Traversenweg absolut"@de , "Absolute crosshead travel"@en ;
        skos:preflabel  "AbsoluteCrossheadTravel"@en .

:Temperature  rdf:type  skos:Concept , owl:Class ;
        rdfs:comment    "Versuche unter kontrollierten Bedingungen müssen bei einer Temperatur von (23 ± 5) °C durchgeführt werden."@de ;
        rdfs:label      "Temperature"@en ;
        skos:altlabel   "Temperature"@en ;
        skos:preflabel  "Temperature"@en .

:CoefficientOfCorrelation
        rdf:type        skos:Concept , owl:Class ;
        rdfs:label      "CoefficientOfCorrelation"@en ;
        skos:altlabel   "coefficient of correlation"@en ;
        skos:preflabel  "CoefficientOfCorrelation"@en .

:TensileStrength  rdf:type  skos:Concept , owl:Class ;
        rdfs:comment    "tensile strength"@en , "maximum amount of tensile (pulling) stress that a material can withstand before failure "@en ;
        rdfs:label      "TensileStrength"@en ;
        skos:altlabel   "tensile strength"@en , "Zugfestigkeit Rm"@de ;
        skos:preflabel  "TensileStrength"@en .

:rollingForce  rdf:type  owl:Class ;
        rdfs:label      "rolling force"@en , "Walzkraft"@de ;
        skos:preflabel  "rolling force"@en , "Walzkraft"@de .

:GrainSize  rdf:type    owl:Class ;
        rdfs:label      "Korngröße"@de , "Grain size"@en ;
        skos:preflabel  "Korngröße"@de , "Grain size"@en .

:hasFailureCriteriaTypeAdd
        rdf:type        owl:ObjectProperty ;
        rdfs:label      "hasFailureCriteriaTypeAdd"@en ;
        rdfs:range      "https://w3id.org/steel/ProcessOntology/FailureCriteriaTypeAdd" ;
        skos:preflabel  "hasFailureCriteriaTypeAdd"@en .

:PoissonRatio  rdf:type    skos:Concept , owl:Class ;
        rdfs:comment       "Poission Ratio to determine the linear elasticity"@en ;
        rdfs:label         "PoissonRatio"@en ;
        rdfs:subClassOf    "https://material-digital.de/pmdco/ValueObject" ;
        skos:altlabel      "PR"@en ;
        skos:preflabel     "PoissonRatio"@en ;
        :UnitLabel         "1" ;
        :hasLabelSourceEn  "LS-DYNA_Manual_Volume_2" .

:hasStrainRateScaleIdendifier
        rdf:type        owl:ObjectProperty ;
        rdfs:label      "hasStrainRateScaleIdendifier"@en ;
        rdfs:range      "https://w3id.org/steel/ProcessOntology/StrainRateScaleIdendifier" ;
        skos:preflabel  "hasStrainRateScaleIdendifier"@en .

:Color  rdf:type        owl:Class ;
        rdfs:comment    "A Color, Green, Yellow, etc.."@en ;
        rdfs:label      "Farbe"@de , "Color"@en ;
        skos:altlabel   "Colour"@en ;
        skos:preflabel  "Farbe"@de , "Color"@en .

:TestPiece  rdf:type    owl:Class ;
        rdfs:comment    "Something that a test is perfomed on"@en ;
        rdfs:label      "Test piece"@en , "Probe"@de ;
        skos:altlabel   "sample, specimen"@en ;
        skos:preflabel  "Test piece"@en , "Probe"@de .

:codeVersion  rdf:type  owl:DatatypeProperty ;
        rdfs:domain     :Code ;
        rdfs:label      "version"@en ;
        rdfs:range      xsd:string ;
        dc:description  "exact version of a code"@en ;
        skos:preflabel  "version"@en .

:Workflow  rdf:type     owl:Class ;
        rdfs:label      "Workflow"@en , "Arbeitsablauf"@de ;
        skos:preflabel  "Workflow"@en , "Arbeitsablauf"@de .

:hasElementDeletionTreatment
        rdf:type        owl:ObjectProperty ;
        rdfs:label      "hasElementDeletionTreatment"@en ;
        rdfs:range      "https://w3id.org/steel/ProcessOntology/ElementDeletionTreatment" ;
        skos:preflabel  "hasElementDeletionTreatment"@en .

:DamageExponent  rdf:type  skos:Concept , owl:Class ;
        rdfs:comment       "Exponent for nonlinear damage accumulation"@en ;
        rdfs:label         "DamageExponent"@en ;
        rdfs:subClassOf    "https://material-digital.de/pmdco/ValueObject" ;
        skos:altlabel      "DMGEXP"@en ;
        skos:preflabel     "DamageExponent"@en ;
        :UnitLabel         "1" ;
        :hasLabelSourceEn  "LS-DYNA_Manual_Volume_2" .

:RValue  rdf:type       skos:Concept , owl:Class ;
        rdfs:label      "RValue"@en ;
        skos:altlabel   "r-value"@en , "r"@de ;
        skos:preflabel  "RValue"@en .

:parameters  rdf:type   owl:DatatypeProperty ;
        rdfs:domain     :Workflow ;
        rdfs:label      "parameters"@en ;
        skos:preflabel  "parameters"@en .

:Experiment  rdf:type   owl:Class ;
        rdfs:label      "Experiment"@en , "Experiment"@de ;
        skos:preflabel  "Experiment"@en , "Experiment"@de .

:PoissonsRatio  rdf:type  skos:Concept , owl:Class ;
        rdfs:label      "PoissonsRatio"@en ;
        skos:altlabel   "poisson`s ratio"@en , "Querkontraktion"@de ;
        skos:preflabel  "PoissonsRatio"@en .

:TestTemperatur  rdf:type  skos:Concept , owl:Class ;
        rdfs:label      "TestTemperatur"@en ;
        skos:altlabel   "temperature"@en , "Prüftemperatur"@de ;
        skos:preflabel  "TestTemperatur"@en .

:DiameterAfterFracture1
        rdf:type        skos:Concept , owl:Class ;
        rdfs:label      "DiameterAfterFracture1"@en ;
        skos:altlabel   "Probendurchmesser nach Bruch D1"@de , "Diameter D1 after fracture"@en ;
        skos:preflabel  "DiameterAfterFracture1"@en .

:Lsdyna  rdf:type        owl:Class ;
        rdfs:comment     "Simulation Software named LSDyna"@en ;
        rdfs:label       "LSDyna"@en , "LSDyna"@de ;
        rdfs:subClassOf  :Solver ;
        skos:preflabel   "LSDyna"@en , "LSDyna"@de .

:hasOutput  rdf:type    owl:ObjectProperty ;
        rdfs:domain     :Code ;
        rdfs:label      "has output"@en ;
        dc:description  "output of a code"@en ;
        skos:preflabel  "has output"@en .

:FailureCriteriaTypeAdd4ElementDeletion
        rdf:type           skos:Concept , owl:Class ;
        rdfs:comment       "Number of time steps that the additional failure criterion must be met before element deletion"@en ;
        rdfs:label         "FailureCriteriaTypeAdd4ElementDeletion"@en ;
        rdfs:subClassOf    "https://material-digital.de/pmdco/ValueObject" ;
        skos:altlabel      "NCYFAIL"@en ;
        skos:preflabel     "FailureCriteriaTypeAdd4ElementDeletion"@en ;
        :UnitLabel         "1" ;
        :hasLabelSourceEn  "LS-DYNA_Manual_Volume_2" .

:LowerYieldStrength  rdf:type  skos:Concept , owl:Class ;
        rdfs:label      "LowerYieldStrength"@en ;
        skos:altlabel   "lower yield strength"@en , "Dehngrenze ReL"@de , "Dehn-/Streckgr. ReL"@de ;
        skos:preflabel  "LowerYieldStrength"@en .

:Plasticity  rdf:type   owl:Class ;
        rdfs:label      "Verformbarkeit"@de , "Plasticity"@en ;
        skos:preflabel  "Verformbarkeit"@de , "Plasticity"@en .

:Strain  rdf:type       skos:Concept , owl:Class ;
        rdfs:comment    "technische Dehnung bezogen auf die Extensometermesslänge"@de ;
        rdfs:label      "Strain"@en , "Dehnung"@de ;
        skos:altlabel   "percentage extension “strain”"@en ;
        skos:preflabel  "Strain"@en , "Dehnung"@de .

:YieldingIdentifier  rdf:type  skos:Concept , owl:Class ;
        rdfs:comment       "Identifier which relates the Load Curve to descibe the yield stress as a function of effective plastic strain.\nIdentifier which relates the Table to descibe the yield stress by using different Load Curves as a function of effective plastic strain and the strain rate (each load curve is related to an individual stain rate)"@en ;
        rdfs:label         "YieldingIdentifier"@en ;
        rdfs:subClassOf    "https://material-digital.de/pmdco/ValueObject" ;
        skos:altlabel      "LCK1"@en , "LCSS"@en ;
        skos:preflabel     "YieldingIdentifier"@en ;
        :UnitLabel         "-" ;
        :hasLabelSourceEn  "LS-DYNA_Manual_Volume_2" .

:Geometry  rdf:type     owl:Class ;
        rdfs:label      "Geometry"@en , "Geometrie"@de ;
        skos:preflabel  "Geometry"@en , "Geometrie"@de .

:WidthAfterFracture2  rdf:type  skos:Concept , owl:Class ;
        rdfs:label      "WidthAfterFracture2"@en ;
        skos:altlabel   "Width B2 after fracture"@en , "Probenbreite B2 nach Bruch"@de ;
        skos:preflabel  "WidthAfterFracture2"@en .

:MeanEngineeringStrainRate
        rdf:type        skos:Concept , owl:Class ;
        rdfs:label      "MeanEngineeringStrainRate"@en ;
        skos:altlabel   "mittlere"@de , "Mean engineering strain rate"@en ;
        skos:preflabel  "MeanEngineeringStrainRate"@en .

:hasTaylorQuinneyCoefficient
        rdf:type        owl:ObjectProperty ;
        rdfs:label      "hasTaylorQuinneyCoefficient"@en ;
        rdfs:range      "https://w3id.org/steel/ProcessOntology/TaylorQuinneyCoefficient" ;
        skos:preflabel  "hasTaylorQuinneyCoefficient"@en .

:TestingRate  rdf:type  skos:Concept , owl:Class ;
        rdfs:comment    "während des Versuchs verwendete Geschwindigkeit(en) als Oberbegriff"@de ;
        rdfs:label      "TestingRate"@en ;
        skos:altlabel   "Testing rate"@en ;
        skos:preflabel  "TestingRate"@en .

:executedBy  rdf:type   owl:DatatypeProperty ;
        rdfs:domain     :Workflow ;
        rdfs:label      "executedBy"@en ;
        skos:preflabel  "executedBy"@en .

:TestingFacility  rdf:type  skos:Concept , owl:Class ;
        rdfs:comment    "Facility that conducted the experiment."@en ;
        rdfs:label      "TestingFacility"@en ;
        skos:altlabel   "Testing facility"@en , "Prüfinstitut"@de ;
        skos:preflabel  "TestingFacility"@en .

:processChainSimulation
        rdf:type  owl:Class .

:TestingDirection  rdf:type  skos:Concept , owl:Class ;
        rdfs:comment    "testing direction related to the rolling direction"@en ;
        rdfs:label      "TestingDirection"@en ;
        skos:altlabel   "testing direction"@en , "Orientierung"@de ;
        skos:preflabel  "TestingDirection"@en .

:ReferenceElementSize
        rdf:type           skos:Concept , owl:Class ;
        rdfs:comment       "Reference element size for which an additional output of damage (and potentially plastic strain) will be generated. This is necessary to ensure the applicability of resulting damage quantities when transferred to different mesh sizes."@en ;
        rdfs:label         "ReferenceElementSize"@en ;
        rdfs:subClassOf    "https://material-digital.de/pmdco/ValueObject" ;
        skos:altlabel      "REFSZ"@en ;
        skos:preflabel     "ReferenceElementSize"@en ;
        :UnitLabel         "mm" ;
        :hasLabelSourceEn  "LS-DYNA_Manual_Volume_2" .

:workRollDiameter  rdf:type  owl:Class ;
        rdfs:label      "work roll diameter"@en , "Arbeitswalzendurchmesser"@de ;
        skos:preflabel  "work roll diameter"@en , "Arbeitswalzendurchmesser"@de .

:YieldForce_0.2Percentage
        rdf:type        skos:Concept , owl:Class ;
        rdfs:label      "YieldForce_0.2Percentage"@en ;
        skos:altlabel   "yield force, 0.2%"@en , "Fp0.2"@de ;
        skos:preflabel  "YieldForce_0.2Percentage"@en .

:Diameter  rdf:type     skos:Concept , owl:Class ;
        rdfs:comment    "The initial diameter of the parallel length"@en ;
        rdfs:label      "Diameter"@en ;
        skos:altlabel   "Probendurchmesser d0"@de , "Diameter"@en ;
        skos:preflabel  "Diameter"@en .

:rollGap  rdf:type      owl:Class ;
        rdfs:label      "roll gap"@en , "Walzspalt"@de ;
        skos:preflabel  "roll gap"@en , "Walzspalt"@de .

:TestingMachine  rdf:type  owl:Class ;
        rdfs:comment    "A machine pervorming an experimental test"@en ;
        rdfs:label      "Testing machine"@en , "Prüfmaschiene"@de ;
        skos:preflabel  "Testing machine"@en , "Prüfmaschiene"@de .

:StressRate  rdf:type   skos:Concept , owl:Class ;
        rdfs:comment    "stress rate"@en ;
        rdfs:label      "StressRate"@en ;
        skos:altlabel   "stress rate"@en , "Geschw."@de ;
        skos:preflabel  "StressRate"@en .

:hasStep  rdf:type      owl:ObjectProperty ;
        rdfs:domain     :DigitalWorkflow ;
        rdfs:label      "has Step"@en ;
        rdfs:range      :WorkflowStep ;
        dc:description  "The relation between digital workflows and workflow steps"@en ;
        skos:preflabel  "has Step"@en .

:Elasticity  rdf:type   owl:Class ;
        rdfs:label      "Elasticity"@en , "Dehnbarkeit"@de ;
        skos:preflabel  "Elasticity"@en , "Dehnbarkeit"@de .

:ElementDeletionTreatment
        rdf:type           skos:Concept , owl:Class ;
        rdfs:comment       "Determines the amount of fully damaged integration points before element deletion:\n>0…Number of integration points which must fail before the element is deleted\n<0…-NUMINT is percentage of integration points/layers which must fail before shell element fails\n=200...Turns off erosion for shells and solids"@en ;
        rdfs:label         "ElementDeletionTreatment"@en ;
        rdfs:subClassOf    "https://material-digital.de/pmdco/ValueObject" ;
        skos:altlabel      "NUMINT"@en ;
        skos:preflabel     "ElementDeletionTreatment"@en ;
        :UnitLabel         "-" ;
        :hasLabelSourceEn  "LS-DYNA_Manual_Volume_2" .

:MatTabulatedJohnsonCook
        rdf:type           skos:Concept , owl:Class ;
        rdfs:comment       "Simple incompressible plasticity model with adiabatic approach"@en ;
        rdfs:label         "MatTabulatedJohnsonCook"@en ;
        rdfs:subClassOf    "https://material-digital.de/pmdco/ValueObject" ;
        skos:altlabel      "Mat224"@en ;
        skos:preflabel     "MatTabulatedJohnsonCook"@en ;
        :hasLabelSourceEn  "LS-DYNA_Manual_Volume_2" .

:MinimumCrosssectionAfterFracture
        rdf:type        skos:Concept , owl:Class ;
        rdfs:comment    "minimum cross-sectional area after fracture"@en ;
        rdfs:label      "MinimumCrosssectionAfterFracture"@en ;
        skos:altlabel   "Su"@de , "Minimum cross-sectional area after fracture"@en , "Bruchquerschnitt Su"@de ;
        skos:preflabel  "MinimumCrosssectionAfterFracture"@en .

:YieldingIdentifierIsoThermal
        rdf:type           skos:Concept , owl:Class ;
        rdfs:comment       "Table ID defining for each temperature value a load curve ID giving the (quasi-static) effective stress versus effective plastic strain for that temperature"@en ;
        rdfs:label         "YieldingIdentifierIsoThermal"@en ;
        rdfs:subClassOf    "https://material-digital.de/pmdco/ValueObject" ;
        skos:altlabel      "LCKT"@en ;
        skos:preflabel     "YieldingIdentifierIsoThermal"@en ;
        :UnitLabel         "-" ;
        :hasLabelSourceEn  "LS-DYNA_Manual_Volume_2" .

:hasMaterialIdentifier
        rdf:type        owl:ObjectProperty ;
        rdfs:label      "hasMaterialIdentifier"@en ;
        rdfs:range      "https://w3id.org/steel/ProcessOntology/MaterialIdentifier" ;
        skos:preflabel  "hasMaterialIdentifier"@en .

:hasFailureStrain  rdf:type  owl:ObjectProperty ;
        rdfs:label      "hasFailureStrain"@en ;
        rdfs:range      "https://w3id.org/steel/ProcessOntology/FailureStrain" ;
        skos:preflabel  "hasFailureStrain"@en .

:PercentagePermanentElongation
        rdf:type        skos:Concept , owl:Class ;
        rdfs:comment    "Zunahme der Anfangsmesslänge (3.1.1) einer Probe nach Entfernen einer festgelegten Zugspannung, angegeben in Prozent, bezogen auf die Anfangsmesslänge (3.1.1)"@de ;
        rdfs:label      "PercentagePermanentElongation"@en ;
        skos:altlabel   "percentage permanent elongation"@en ;
        skos:preflabel  "PercentagePermanentElongation"@en .

:stand  rdf:type        owl:Class ;
        rdfs:label      "stand"@en , "Walzgerüst"@de ;
        skos:preflabel  "stand"@en , "Walzgerüst"@de .

:NominalEngineeringStrainRate
        rdf:type        skos:Concept , owl:Class ;
        rdfs:label      "NominalEngineeringStrainRate"@en ;
        skos:altlabel   "nominell"@de , "Nominal engineering strain rate"@en ;
        skos:preflabel  "NominalEngineeringStrainRate"@en .

:TrueStress  rdf:type   skos:Concept , owl:Class ;
        rdfs:label      "TrueStress"@en , "True Stress"@en , "wahre Spannung"@de ;
        skos:altlabel   "true stress"@en , "Sigw(dL)"@de ;
        skos:preflabel  "True Stress"@en , "TrueStress"@en , "wahre Spannung"@de .

:Preload  rdf:type      skos:Concept , owl:Class ;
        rdfs:comment    "Um ein Ausrichten der Probe in der Einspannvorrichtung zu erreichen, darf eine Vorkraft aufgebracht werden, die 5 % des spezifizierten oder zu erwartenden Streckgrenzenwertes nicht überschreitet. Eine Korrektur der Dehnung sollte unter Berücksichtigung der Vorkraft vorgenommen werden."@de ;
        rdfs:label      "Preload"@en ;
        skos:preflabel  "Preload"@en .

:MassDensity  rdf:type     skos:Concept , owl:Class ;
        rdfs:comment       "Mass densisty of the material"@en ;
        rdfs:label         "MassDensity"@en ;
        rdfs:subClassOf    "https://material-digital.de/pmdco/ValueObject" ;
        skos:altlabel      "RO"@en ;
        skos:preflabel     "MassDensity"@en ;
        :UnitLabel         "g/cm^3" ;
        :hasLabelSourceEn  "LS-DYNA_Manual_Volume_2" .

:DamageThreshold  rdf:type  skos:Concept , owl:Class ;
        rdfs:comment       "Damage threshold value (critical damage). If a load curve of critical plastic strain or fixed value is given by ECRIT, input is ignored."@en ;
        rdfs:label         "DamageThreshold"@en ;
        rdfs:subClassOf    "https://material-digital.de/pmdco/ValueObject" ;
        skos:altlabel      "DCRIT"@en ;
        skos:preflabel     "DamageThreshold"@en ;
        :UnitLabel         "1" ;
        :hasLabelSourceEn  "LS-DYNA_Manual_Volume_2" .

:hasFadingExponent  rdf:type  owl:ObjectProperty ;
        rdfs:label      "hasFadingExponent"@en ;
        rdfs:range      "https://w3id.org/steel/ProcessOntology/FadingExponent" ;
        skos:preflabel  "hasFadingExponent"@en .

:StrainRateFormulationFlag
        rdf:type           skos:Concept , owl:Class ;
        rdfs:comment       "Flag which determines the treatment of strain rate to evaluate yielding:\n=-1.0: Cowper-Symonds with effective deviatoric rate rather than total\n=0.0: Scale yield stress (default)\n=1.0: Viscoplastic formulation\n=3.0: Same as VP = 0, but with filtered effective total strain rates"@en ;
        rdfs:label         "StrainRateFormulationFlag"@en ;
        rdfs:subClassOf    "https://material-digital.de/pmdco/ValueObject" ;
        skos:altlabel      "VP"@en ;
        skos:preflabel     "StrainRateFormulationFlag"@en ;
        :hasLabelSourceEn  "LS-DYNA_Manual_Volume_2" .

:PyironNotebook  rdf:type  owl:Class ;
        rdfs:comment    "Jupyter Pyiron Notebook"@en ;
        rdfs:label      "Pyiron notebook"@en , "Pyiron Notebook"@de ;
        skos:preflabel  "Pyiron notebook"@en , "Pyiron Notebook"@de .

:DiameterAfterFracture2
        rdf:type        skos:Concept , owl:Class ;
        rdfs:label      "DiameterAfterFracture2"@en ;
        skos:altlabel   "Probendurchmesser nach Bruch D2"@de , "Diameter D2 after fracture"@en ;
        skos:preflabel  "DiameterAfterFracture2"@en .

:TaylorQuinneyCoefficient
        rdf:type           skos:Concept , owl:Class ;
        rdfs:comment       "Determines the fraction of plastic work converted into heat:\n<0…|BETA|->load curve for temperature dependend BETA\n>0…constant value is used"@en ;
        rdfs:label         "TaylorQuinneyCoefficient"@en ;
        rdfs:subClassOf    "https://material-digital.de/pmdco/ValueObject" ;
        skos:altlabel      "BETA"@en ;
        skos:preflabel     "TaylorQuinneyCoefficient"@en ;
        :UnitLabel         "1" ;
        :hasLabelSourceEn  "LS-DYNA_Manual_Volume_2" .

:MaximumForce  rdf:type  skos:Concept , owl:Class ;
        rdfs:comment    "highest force that the test piece withstands during the test"@en ;
        rdfs:label      "MaximumForce"@en ;
        skos:altlabel   "maximum force"@en , "Höchstzugkraft Fm"@de ;
        skos:preflabel  "MaximumForce"@en .

:UpperYieldStrength  rdf:type  skos:Concept , owl:Class ;
        rdfs:label      "UpperYieldStrength"@en ;
        skos:altlabel   "upper yield strength"@en ;
        skos:preflabel  "UpperYieldStrength"@en .

:SampleIdentifier  rdf:type  skos:Concept , owl:Class ;
        rdfs:comment    "Unique ID (IWM intern)"@en ;
        rdfs:label      "SampleIdentifier"@en ;
        skos:altlabel   "Sample identifier"@en , "Probennummer"@de , "Proben-Nr."@de ;
        skos:preflabel  "SampleIdentifier"@en .

:MaximumForceDiscontinousYielding
        rdf:type        skos:Concept , owl:Class ;
        rdfs:label      "MaximumForceDiscontinousYielding"@en ;
        skos:altlabel   "maximum force \"discontinous yielding\""@en ;
        skos:preflabel  "MaximumForceDiscontinousYielding"@en .

:StrainRate  rdf:type   skos:Concept , owl:Class ;
        rdfs:comment    "strain rate either of the parallel length or of the gauge length/extensometer length (should be specified)"@en , "the rate at which a material deforms under applied stress. It is a measure of how quickly the material's shape or dimensions change in response to external forces, such as tension, compression, or shear. Strain rate is typically expressed in units of inverse time (e.g., s^-1 or min^-1)."@en ;
        rdfs:label      "StrainRate"@en ;
        skos:altlabel   "strain rate"@en , "Strain Rate"@en , "Dehngeschwindigkeit"@de ;
        skos:preflabel  "StrainRate"@en .

:MinTimeStep4ElementDel
        rdf:type           skos:Concept , owl:Class ;
        rdfs:comment       "Minimum time step size for automatic element deletion"@en ;
        rdfs:label         "MinTimeStep4ElementDel"@en ;
        rdfs:subClassOf    "https://material-digital.de/pmdco/ValueObject" ;
        skos:altlabel      "TDEL"@en ;
        skos:preflabel     "MinTimeStep4ElementDel"@en ;
        :UnitLabel         "s" ;
        :hasLabelSourceEn  "LS-DYNA_Manual_Volume_2" .

:PercentagePlasticExtensionAtMaximumForce
        rdf:type        skos:Concept , owl:Class ;
        rdfs:comment    "uniform elongation"@en ;
        rdfs:label      "PercentagePlasticExtensionAtMaximumForce"@en ;
        skos:altlabel   "percentage plastic extension at maximum force"@en , "Gleichmaßdehnung Ag"@de , "Dehnung bei Höchstkraft Ag"@de ;
        skos:preflabel  "PercentagePlasticExtensionAtMaximumForce"@en .

:usesCode  rdf:type     owl:ObjectProperty ;
        rdfs:domain     :Job ;
        rdfs:label      "uses Code"@en ;
        rdfs:range      :Code ;
        dc:description  "code used by a job"@en ;
        skos:preflabel  "uses Code"@en .

:Machine  rdf:type      skos:Concept , owl:Class ;
        rdfs:comment    "Data of the machine used for the experiment."@en , "Die Prüfmaschine sollte mit einer analogen Messwertausgabe, die nicht durch die Software beeinflusst wird, ausgerüstet sein. Ist eine solche Ausgabe nicht vorgesehen, sollten digitale Rohdaten ausgegeben werden können. Der Prüfmaschinenhersteller sollte Auskunft über die Erzeugung der digitalen Rohdaten und ihre Verarbeitung durch die Software geben. Die Rohdaten sollten in SI-Einheiten angegeben werden und sich auf die Kraft, die Verlängerung (der Extensometer-Messlänge), den Traversenweg, die Zeit und die Probenmaße beziehen. Ein Beispiel eines geeigneten Datenformats ist in Bild A.1 dargestellt."@de ;
        rdfs:label      "Machine"@en ;
        skos:altlabel   "Testing Machine"@en , "Machine data"@en , "Prüfmaschine"@de , "Prüfmasch."@de , "Maschinendaten"@de , "Machine"@en ;
        skos:preflabel  "Machine"@en .

:GrainBoundaries  rdf:type  owl:Class ;
        rdfs:comment    "need at least two grains"@en ;
        rdfs:label      "grain boundaries"@en , "Korngrenzen"@de ;
        skos:preflabel  "grain boundaries"@en , "Korngrenzen"@de .

:Damage  rdf:type       owl:Class ;
        rdfs:label      "Schaden"@de , "Damage"@en ;
        skos:preflabel  "Schaden"@de , "Damage"@en .

:JobOutput  rdf:type    owl:Class ;
        rdfs:comment    "the output parameter for a pyiron job"@en ;
        rdfs:label      "Pyiron job output"@en , "Job-Output-Parameter"@de ;
        skos:preflabel  "Pyiron job output"@en , "Job-Output-Parameter"@de .

:rollingDirection  rdf:type  owl:Class ;
        rdfs:label      "rolling direction"@en , "Walzrichtung"@de ;
        skos:altlabel   "RD"@en ;
        skos:preflabel  "rolling direction"@en , "Walzrichtung"@de .

:hasFailureStrainIdentifier
        rdf:type        owl:ObjectProperty ;
        rdfs:label      "hasFailureStrainIdentifier"@en ;
        rdfs:range      "https://w3id.org/steel/ProcessOntology/FailureStrainIdentifier" ;
        skos:preflabel  "hasFailureStrainIdentifier"@en .

:FailureStrainIdentifier4Temperature
        rdf:type           skos:Concept , owl:Class ;
        rdfs:comment       "Load curve ID defining plastic failure strain as a function of temperature"@en ;
        rdfs:label         "FailureStrainIdentifier4Temperature"@en ;
        rdfs:subClassOf    "https://material-digital.de/pmdco/ValueObject" ;
        skos:altlabel      "LCH"@en ;
        skos:preflabel     "FailureStrainIdentifier4Temperature"@en ;
        :UnitLabel         "-" ;
        :hasLabelSourceEn  "LS-DYNA_Manual_Volume_2" .

:hasMatTabulatedJohnsonCook
        rdf:type        owl:ObjectProperty ;
        rdfs:label      "hasMatTabulatedJohnsonCook"@en ;
        rdfs:range      "https://w3id.org/steel/ProcessOntology/MatTabulatedJohnsonCook" ;
        skos:preflabel  "hasMatTabulatedJohnsonCook"@en .

:Solver  rdf:type       owl:Class ;
        rdfs:comment    "A software for solving compelex lin-diff equations, Like Abaqus or Lsdyna"@en ;
        rdfs:label      "Solver"@en , "Solver"@de ;
        skos:altlabel   "Gleichungslöser"@de ;
        skos:preflabel  "Solver"@en , "Solver"@de .

:jobStartTime  rdf:type  owl:DatatypeProperty ;
        rdfs:domain     :Job ;
        rdfs:label      "start time"@en ;
        rdfs:range      xsd:dateTime ;
        dc:description  "time and date when the execution of a job instance was started"@en ;
        skos:preflabel  "start time"@en .

:ForceMeasuringDevice
        rdf:type        owl:Class , skos:Concept ;
        rdfs:comment    "Die Kraftmesseinrichtung der Zugprüfmaschine muss im relevanten Bereich mindestens der Klasse 1 nach ISO 7500-1 entsprechen."@de , "Genauigkeit der Prüfeinrichtungen: Die Kraftmesseinrichtung der Prüfmaschine muss mindestens der Klasse 1 nach ISO 7500-1 entsprechen."@de , "Type of the force transducer. (description replaced by Zugversuch Instron)"@en , "Type of the force measurement (force transducer, strain gauges, ....)"@en ;
        rdfs:label      "ForceMeasuringDevice"@en ;
        skos:altlabel   "Kraftaufnehmer"@de , "Force transducer"@en , "force-measuring device"@en , "Force-measuring device"@en , "Kraftmesseinrichtung"@de , "Force-measuring system"@en ;
        skos:preflabel  "ForceMeasuringDevice"@en .

:hasPrincipalStressLimit4PostProcessing
        rdf:type        owl:ObjectProperty ;
        rdfs:label      "hasPrincipalStressLimit4PostProcessing"@en ;
        rdfs:range      "https://w3id.org/steel/ProcessOntology/PrincipalStressLimit4PostProcessing" ;
        skos:preflabel  "hasPrincipalStressLimit4PostProcessing"@en .

:FinalThickness  rdf:type  owl:Class ;
        rdfs:label      "final thickness"@en , "Enddicke"@de ;
        skos:preflabel  "final thickness"@en , "Enddicke"@de .

:hasMassDensity  rdf:type  owl:ObjectProperty ;
        rdfs:label      "hasMassDensity"@en ;
        rdfs:range      "https://w3id.org/steel/ProcessOntology/MassDensity" ;
        skos:preflabel  "hasMassDensity"@en .

:ForceMeasuringSystem
        rdf:type        skos:Concept , owl:Class ;
        rdfs:comment    "Measuring system for measurement of force"@en ;
        rdfs:label      "ForceMeasuringSystem"@en ;
        skos:altlabel   "Kraft"@de , "Force measurement system"@en ;
        skos:preflabel  "ForceMeasuringSystem"@en .

:stripWidth  rdf:type   owl:Class ;
        rdfs:label      "strip width"@en , "Bandbreite"@de ;
        skos:preflabel  "strip width"@en , "Bandbreite"@de .
